specs/Spec.Agile.HPKE.fst
@@ -23,12 +23,11 @@ let pow2_35_less_than_pow2_125 : _:unit{pow2 32 * pow2 3 <= pow2 125 - 1} = asse
 
 /// Types
 
-// TODO This must match the first two and set the id accordingly
 val id_kem: cs:ciphersuite -> Tot (lbytes 2)
-let id_kem cs = let dh, _, _, _ = cs in
-  match dh with
-  | DH.DH_P256 -> create 1 (u8 0) @| create 1 (u8 16)
-  | DH.DH_Curve25519 -> create 1 (u8 0) @| create 1 (u8 32)
+let id_kem cs = let kem_dh, kem_hash, _, _ = cs in
+  match kem_dh, kem_hash with
+  | DH.DH_P256, Hash.SHA2_256 -> create 1 (u8 0) @| create 1 (u8 16)
+  | DH.DH_Curve25519, Hash.SHA2_256 -> create 1 (u8 0) @| create 1 (u8 32)
 
 val id_kdf: cs:ciphersuite -> Tot (lbytes 2)
 let id_kdf cs = let _, _, _, h = cs in
@@ -44,10 +43,14 @@ let id_aead cs = let _, _, a, _ = cs in
   | AEAD.AES256_GCM -> create 1 (u8 0) @| create 1 (u8 2)
   | AEAD.CHACHA20_POLY1305 -> create 1 (u8 0) @| create 1 (u8 3)
 
+val suite_id_kem: cs:ciphersuite -> Tot (lbytes size_suite_id_kem)
+let suite_id_kem cs =
+  Seq.append label_KEM (id_kem cs)
 
-val id_of_cs: cs:ciphersuite -> Tot (lbytes size_cs_identifier)
+val suite_id_hpke: cs:ciphersuite -> Tot (lbytes size_suite_id_hpke)
 // TODO This should already be in big endian each
-let id_of_cs cs = id_kem cs @| id_kdf cs @| id_aead cs
+let suite_id_hpke cs =
+  Seq.append label_HPKE (id_kem cs @| id_kdf cs @| id_aead cs)
 
 val id_of_mode: m:mode -> Tot (lbytes size_mode_identifier)
 let id_of_mode m =
@@ -67,61 +70,53 @@ let id_of_mode m =
 //= ()
 ////  assert (Seq.length label_rfcXXXX + Seq.length label + Seq.length ikm + Spec.Hash.Definitions.block_length a + consts <= Spec.Hash.Definitions.max_input_length a) by (FStar.Tactics.fail "foobar")
 
-let labeled_extract a salt label ikm =
+let labeled_extract a suite_id salt label ikm =
 //  labeled_extract_pred_ikm_elim a label ikm 0;
-  let labeledIKM = Seq.append label_rfcXXXX label in
-  let labeledIKM = Seq.append labeledIKM ikm in
-  HKDF.extract a salt labeledIKM
+  let labeled_ikm1 = Seq.append label_rfcXXXX suite_id in
+  let labeled_ikm2 = Seq.append labeled_ikm1 label in
+  let labeled_ikm3 = Seq.append labeled_ikm2 ikm in
+  HKDF.extract a salt labeled_ikm3
 
-let labeled_expand a prk label info l =
-  let labeledInfo = nat_to_bytes_be 2 l in
-  let labeledInfo = Seq.append labeledInfo label_rfcXXXX in
-  let labeledInfo = Seq.append labeledInfo label in
-  let labeledInfo = Seq.append labeledInfo info in
-  HKDF.expand a prk labeledInfo l
+let labeled_expand a suite_id prk label info l =
+  let labeled_info1 = nat_to_bytes_be 2 l in
+  let labeled_info2 = Seq.append labeled_info1 label_rfcXXXX in
+  let labeled_info3 = Seq.append labeled_info2 suite_id in
+  let labeled_info4 = Seq.append labeled_info3 label in
+  let labeled_info5 = Seq.append labeled_info4 info in
+  HKDF.expand a prk labeled_info5 l
 
 let extract_and_expand_dh_pred (cs:ciphersuite) (dh_length:nat) =
-  labeled_extract_ikm_length_pred (kem_hash_of_cs cs) (Seq.length label_dh + dh_length)
+  labeled_extract_ikm_length_pred (kem_hash_of_cs cs) (size_suite_id_kem + Seq.length label_eae_prk + dh_length)
 
 let extract_and_expand_ctx_pred (cs:ciphersuite) (ctx_length:nat) =
-  labeled_expand_info_length_pred (kem_hash_of_cs cs) (Seq.length label_prk + ctx_length)
+  labeled_expand_info_length_pred (kem_hash_of_cs cs) (size_suite_id_kem + Seq.length label_shared_secret + ctx_length)
 
 val extract_and_expand:
     cs:ciphersuite
   -> dh:bytes
-  -> kemContext:bytes ->
+  -> kem_context:bytes ->
   Pure (key_kem_s cs)
     (requires
       extract_and_expand_dh_pred cs (Seq.length dh) /\
-      extract_and_expand_ctx_pred cs (Seq.length kemContext))
+      extract_and_expand_ctx_pred cs (Seq.length kem_context))
     (ensures fun _ -> True)
 
-let extract_and_expand cs dh kemContext =
-  let prk = labeled_extract (kem_hash_of_cs cs) lbytes_empty label_dh dh in
-  labeled_expand (kem_hash_of_cs cs) prk label_prk kemContext (size_kem_key cs)
+let extract_and_expand cs dh kem_context =
+  let eae_prk = labeled_extract (kem_hash_of_cs cs) (suite_id_kem cs) lbytes_empty label_eae_prk dh in
+  labeled_expand (kem_hash_of_cs cs) (suite_id_kem cs) eae_prk label_shared_secret kem_context (size_kem_key cs)
 
-let unmarshal cs pk = match curve_of_cs cs with
+let deserialize cs pk = match curve_of_cs cs with
   | DH.DH_Curve25519 -> pk
   // Extract the point coordinates by removing the first representation byte
   | DH.DH_P256 -> sub pk 1 64
 
 
-let marshal cs pk = match curve_of_cs cs with
+let serialize cs pk = match curve_of_cs cs with
   | DH.DH_Curve25519 -> pk
   // Add the first representation byte to the point coordinates
   | DH.DH_P256 -> create 1 (u8 4) @| pk
 
 
-/// def Encap(pkR):
-///   skE, pkE = GenerateKeyPair()
-///   dh = DH(skE, pkR)
-///   enc = Marshal(pkE)
-///
-///   pkRm = Marshal(pkR)
-///   kemContext = concat(enc, pkRm)
-///
-///  zz = ExtractAndExpand(dh, kemContext)
-///  return zz, enc
 
 val encap:
     cs:ciphersuite
@@ -134,27 +129,18 @@ let encap cs skE pkR =
   match DH.secret_to_public (curve_of_cs cs) skE with
   | None -> None
   | Some pkE ->
-    let enc = marshal cs pkE in
+    let enc = serialize cs pkE in
     match DH.dh (curve_of_cs cs) skE pkR with
     | None -> None
     | Some dh ->
-      let pkRm = marshal cs pkR in
-      let kemContext:lbytes (2*size_dh_public cs) = concat enc pkRm in
-      let dhm = marshal cs dh in
-      assert (Seq.length enc + Seq.length pkRm = Seq.length kemContext);
+      let pkRm = serialize cs pkR in
+      let kem_context:lbytes (2*size_dh_public cs) = concat enc pkRm in
+      let dhm = serialize cs dh in
+      assert (Seq.length enc + Seq.length pkRm = Seq.length kem_context);
       assert (extract_and_expand_ctx_pred cs (Seq.length enc + Seq.length pkRm));
-      let zz:key_kem_s cs = extract_and_expand cs dhm kemContext in
-      Some (zz, enc)
+      let shared_secret:key_kem_s cs = extract_and_expand cs dhm kem_context in
+      Some (shared_secret, enc)
 
-/// def Decap(enc, skR):
-///   pkE = Unmarshal(enc)
-///   dh = DH(skR, pkE)
-/// 
-///   pkRm = Marshal(pk(skR))
-///   kemContext = concat(enc, pkRm)
-/// 
-///   zz = ExtractAndExpand(dh, kemContext)
-///   return zz
 
 val decap:
     cs: ciphersuite
@@ -164,34 +150,23 @@ val decap:
 
 #set-options "--z3rlimit 150 --fuel 0 --ifuel 2"
 let decap cs enc skR =
-  let pkE = unmarshal cs enc in
+  let pkE = deserialize cs enc in
   match DH.dh (curve_of_cs cs) skR pkE with
   | None -> None
   | Some dh ->
     match DH.secret_to_public (curve_of_cs cs) skR with
     | None -> None
     | Some pkR ->
-      let pkRm = marshal cs pkR in
-      let kemContext:lbytes (2*size_dh_public cs) = concat enc pkRm in
-      let dhm = marshal cs dh in
-      assert (Seq.length enc + Seq.length pkRm = Seq.length kemContext);
-      assert (extract_and_expand_ctx_pred cs (Seq.length kemContext));
-      let zz = extract_and_expand cs dhm kemContext in
-      Some (zz)
+      let pkRm = serialize cs pkR in
+      let kem_context:lbytes (2*size_dh_public cs) = concat enc pkRm in
+      let dhm = serialize cs dh in
+      assert (Seq.length enc + Seq.length pkRm = Seq.length kem_context);
+      assert (extract_and_expand_ctx_pred cs (Seq.length kem_context));
+      let shared_secret = extract_and_expand cs dhm kem_context in
+      Some (shared_secret)
 
 // TODO Correctness lemma for encap/decap?
 
-/// def AuthEncap(pkR, skS):
-///   skE, pkE = GenerateKeyPair()
-///   dh = concat(DH(skE, pkR), DH(skS, pkR))
-///   enc = Marshal(pkE)
-///
-///   pkRm = Marshal(pkR)
-///   pkSm = Marshal(pk(skS))
-///   kemContext = concat(enc, pkRm, pkSm)
-///
-///   zz = ExtractAndExpand(dh, kemContext)
-///   return zz, enc
 
 val auth_encap:
     cs:ciphersuite
@@ -211,33 +186,23 @@ let auth_encap cs skE pkR skS =
       match DH.dh (curve_of_cs cs) skS pkR with
       | None -> None
       | Some ss ->
-        let esm = marshal cs es in
-        let ssm = marshal cs ss in
+        let esm = serialize cs es in
+        let ssm = serialize cs ss in
         let dh = concat esm ssm in
-        let enc = marshal cs pkE in
-        match DH.secret_to_public (curve_of_cs cs) skE with
+        let enc = serialize cs pkE in
+        match DH.secret_to_public (curve_of_cs cs) skS with
         | None -> None
         | Some pkS ->
-          let pkSm = marshal cs pkS in
-          let pkRm = marshal cs pkR in
-          let kemContext:lbytes (3*size_dh_public cs) = concat enc (concat pkRm pkSm) in
-          assert (Seq.length enc + Seq.length pkRm + Seq.length pkSm = Seq.length kemContext);
-          assert (extract_and_expand_ctx_pred cs (Seq.length kemContext));
+          let pkSm = serialize cs pkS in
+          let pkRm = serialize cs pkR in
+          let kem_context:lbytes (3*size_dh_public cs) = concat enc (concat pkRm pkSm) in
+          assert (Seq.length enc + Seq.length pkRm + Seq.length pkSm = Seq.length kem_context);
+          assert (extract_and_expand_ctx_pred cs (Seq.length kem_context));
           assert (Seq.length dh = 2*size_dh_public cs);
           assert (extract_and_expand_dh_pred cs (Seq.length dh));
-          let zz = extract_and_expand cs dh kemContext in
-          Some (zz, enc)
+          let shared_secret = extract_and_expand cs dh kem_context in
+          Some (shared_secret, enc)
 
-/// def AuthDecap(enc, skR, pkS):
-///   pkE = Unmarshal(enc)
-///   dh = concat(DH(skR, pkE), DH(skR, pkS))
-///
-///   pkRm = Marshal(pk(skR))
-///   pkSm = Marshal(pkS)
-///   kemContext = concat(enc, pkRm, pkSm)
-///
-///   zz = ExtractAndExpand(dh, kemContext)
-///   return zz
 
 val auth_decap:
     cs: ciphersuite
@@ -248,42 +213,40 @@ val auth_decap:
 
 #set-options "--z3rlimit 150 --fuel 0 --ifuel 2"
 let auth_decap cs enc skR pkS =
-  let pkE = unmarshal cs enc in
+  let pkE = deserialize cs enc in
   match DH.dh (curve_of_cs cs) skR pkE with
   | None -> None
   | Some es ->
     match DH.dh (curve_of_cs cs) skR pkS with
     | None -> None
     | Some ss ->
-      let esm = marshal cs es in
-      let ssm = marshal cs ss in
+      let esm = serialize cs es in
+      let ssm = serialize cs ss in
       let dh = concat esm ssm in
-      let enc = marshal cs pkE in
+      let enc = serialize cs pkE in
       match DH.secret_to_public (curve_of_cs cs) skR with
       | None -> None
       | Some pkR ->
-        let pkRm = marshal cs pkR in
-        let pkSm = marshal cs pkS in
-        let kemContext:lbytes (3*size_dh_public cs) = concat enc (concat pkRm pkSm) in
-        assert (Seq.length enc + Seq.length pkRm + Seq.length pkSm = Seq.length kemContext);
-        assert (extract_and_expand_ctx_pred cs (Seq.length kemContext));
+        let pkRm = serialize cs pkR in
+        let pkSm = serialize cs pkS in
+        let kem_context:lbytes (3*size_dh_public cs) = concat enc (concat pkRm pkSm) in
+        assert (Seq.length enc + Seq.length pkRm + Seq.length pkSm = Seq.length kem_context);
+        assert (extract_and_expand_ctx_pred cs (Seq.length kem_context));
         assert (Seq.length dh = 2*size_dh_public cs);
         assert (extract_and_expand_dh_pred cs (Seq.length dh));
-        let zz = extract_and_expand cs dh kemContext in
-        Some (zz)
-
-/// default_psk = zero(0)
-/// default_pskId = zero(0)
-
-let default_psk (cs:ciphersuite):psk_s cs  = create (size_kdf cs) (u8 0)
-//let default_psk (cs:ciphersuite):psk_s cs  = lbytes_empty // TODO change as soon as test vectors have been updated
-//let default_pskID (cs:ciphersuite):pskID_s cs = lbytes_empty
-let default_pskID (cs:ciphersuite):pskID_s cs = create (size_kdf cs) (u8 0)
+        let shared_secret = extract_and_expand cs dh kem_context in
+        Some (shared_secret)
 
 
-/// def VerifyPSKInputs(mode, psk, pskID):
+//let default_psk (cs:ciphersuite):psk_s cs  = create (size_kdf cs) (u8 0)
+//let default_psk_id (cs:ciphersuite):psk_id_s cs = create (size_kdf cs) (u8 0)
+let default_psk = lbytes_empty
+let default_psk_id = lbytes_empty
+
+
+/// def VerifyPSKInputs(mode, psk, psk_id):
 ///   got_psk = (psk != default_psk)
-///   if got_psk != (pskID != default_pskID):
+///   if got_psk != (psk_id != default_psk_id):
 ///     raise Exception("Inconsistent PSK inputs")
 ///
 ///   if got_psk and (mode in [mode_base, mode_auth]):
@@ -297,13 +260,13 @@ let default_pskID (cs:ciphersuite):pskID_s cs = create (size_kdf cs) (u8 0)
 val build_context:
     cs:ciphersuite
   -> m:mode
-  -> pskID_hash:lbytes (size_kdf cs)
+  -> psk_id_hash:lbytes (size_kdf cs)
   -> info_hash:lbytes (size_kdf cs) ->
   Tot (lbytes (size_ks_ctx cs))
 
-let build_context cs m pskID_hash info_hash =
-  let context = (id_of_cs cs) @| (id_of_mode m) in
-  let context = Seq.append context pskID_hash in
+let build_context cs m psk_id_hash info_hash =
+  let context = id_of_mode m in
+  let context = Seq.append context psk_id_hash in
   let context = Seq.append context info_hash in
   context
 
@@ -316,11 +279,11 @@ let lbytes_equal (#l1:nat) (#l2:size_nat) (b1:bytes{Seq.length b1 = l1}) (b2:lby
   lbytes_eq #l2 b1 b2
 
 (* // TODO use heterogenous equality *)
-(* // TODO replace got_psk and got_pskID by match on an option type? *)
-(* let verify_psk_inputs (cs:ciphersuite) (m:mode) (psk:psk_s cs) (pskID:pskID_s cs) : bool = *)
+(* // TODO replace got_psk and got_psk_id by match on an option type? *)
+(* let verify_psk_inputs (cs:ciphersuite) (m:mode) (psk:psk_s cs) (psk_id:psk_id_s cs) : bool = *)
 (*   let got_psk = not (lbytes_equal #(Seq.length psk) #(size_kdf cs) psk (default_psk cs)) in *)
-(*   let got_pskID = not (lbytes_equal #(Seq.length pskID) #0 pskID (default_pskID cs)) in *)
-(*   if not (got_psk = got_pskID) then false else // Inconsistent PSK inputs *)
+(*   let got_psk_id = not (lbytes_equal #(Seq.length psk_id) #0 psk_id (default_psk_id cs)) in *)
+(*   if not (got_psk = got_psk_id) then false else // Inconsistent PSK inputs *)
 (*   match (m, got_psk) with *)
 (*   | (Base, true) -> false     // PSK input provided when not needed *)
 (*   | (Auth, true) -> false     // PSK input provided when not needed *)
@@ -328,7 +291,7 @@ let lbytes_equal (#l1:nat) (#l2:size_nat) (b1:bytes{Seq.length b1 = l1}) (b2:lby
 (*   | (AuthPSK, false) -> false // Missing required PSK input *)
 (*   | _ -> true *)
 
-let verify_psk_inputs (cs:ciphersuite) (m:mode) (opsk:option(psk_s cs & pskID_s cs)) : bool =
+let verify_psk_inputs (cs:ciphersuite) (m:mode) (opsk:option(psk_s cs & psk_id_s cs)) : bool =
   match (m, opsk) with
   | Base, None -> true
   | PSK, Some _ -> true
@@ -339,27 +302,26 @@ let verify_psk_inputs (cs:ciphersuite) (m:mode) (opsk:option(psk_s cs & pskID_s 
 val key_schedule:
     cs:ciphersuite
   -> m:mode
-  -> zz:key_kem_s cs
+  -> shared_secret:key_kem_s cs
   -> info:info_s cs
-  -> opsk:option (psk_s cs & pskID_s cs) ->
+  -> opsk:option (psk_s cs & psk_id_s cs) ->
   Pure (encryption_context cs)
     (requires verify_psk_inputs cs m opsk)
     (ensures fun _ -> True)
 
-let key_schedule cs m zz info opsk =
-  let (psk, pskID) =
+let key_schedule cs m shared_secret info opsk =
+  let (psk, psk_id) =
     match opsk with
-    | None -> (default_psk cs, default_pskID cs)
-    | Some (psk, pskID) -> (psk, pskID) in
-  let pskID_hash = labeled_extract (hash_of_cs cs) lbytes_empty label_pskID_hash pskID in
-  let info_hash = labeled_extract (hash_of_cs cs) lbytes_empty label_info_hash info in
-  let context = build_context cs m pskID_hash info_hash in
-  let psk_hash = labeled_extract (hash_of_cs cs) lbytes_empty label_psk_hash psk in
-  let secret = labeled_extract (hash_of_cs cs) psk_hash label_secret zz in
-  let key = labeled_expand (hash_of_cs cs) secret label_key context (size_aead_key cs) in
-  let nonce = labeled_expand (hash_of_cs cs) secret label_nonce context (size_aead_nonce cs) in
-  let exporter_secret = labeled_expand (hash_of_cs cs) secret label_exp context (size_kdf cs) in
-  (key, nonce, 0, exporter_secret)
+    | None -> (default_psk, default_psk_id)
+    | Some (psk, psk_id) -> (psk, psk_id) in
+  let psk_id_hash = labeled_extract (hash_of_cs cs) (suite_id_hpke cs) lbytes_empty label_psk_id_hash psk_id in
+  let info_hash = labeled_extract (hash_of_cs cs) (suite_id_hpke cs) lbytes_empty label_info_hash info in
+  let context = build_context cs m psk_id_hash info_hash in
+  let secret = labeled_extract (hash_of_cs cs) (suite_id_hpke cs) shared_secret label_secret psk in
+  let key = labeled_expand (hash_of_cs cs) (suite_id_hpke cs) secret label_key context (size_aead_key cs) in
+  let base_nonce = labeled_expand (hash_of_cs cs) (suite_id_hpke cs) secret label_base_nonce context (size_aead_nonce cs) in
+  let exporter_secret = labeled_expand (hash_of_cs cs) (suite_id_hpke cs) secret label_exp context (size_kdf cs) in
+  (key, base_nonce, 0, exporter_secret)
 
 let key_of_ctx (cs:ciphersuite) (ctx:encryption_context cs) =
   let key, _, _, _ = ctx in key
@@ -379,7 +341,7 @@ let set_seq (cs:ciphersuite) (ctx:encryption_context cs) (seq:seq_aead_s cs) =
 
 let context_export cs ctx exp_ctx l =
   let exp_sec = exp_sec_of_ctx cs ctx in
-  labeled_expand (hash_of_cs cs) exp_sec label_sec exp_ctx l
+  labeled_expand (hash_of_cs cs) (suite_id_hpke cs) exp_sec label_sec exp_ctx l
 
 
 let context_compute_nonce cs ctx seq =
@@ -416,26 +378,26 @@ let context_open cs ctx aad ct =
 
 /// def SetupBaseS(pkR, info):
 ///   zz, enc = Encap(pkR)
-///   return enc, KeySchedule(mode_base, zz, info, default_psk, default_pskID)
+///   return enc, KeySchedule(mode_base, zz, info, default_psk, default_psk_id)
 
 let setupBaseS cs skE pkR info =
   match encap cs skE pkR with
   | None -> None
-  | Some (zz, enc) ->
-    let enc_ctx = key_schedule cs Base zz info None in
+  | Some (shared_secret, enc) ->
+    let enc_ctx = key_schedule cs Base shared_secret info None in
     Some (enc, enc_ctx)
 
 
 /// def SetupBaseR(enc, skR, info):
 ///   zz = Decap(enc, skR)
-///   return KeySchedule(mode_base, zz, info, default_psk, default_pskID)
+///   return KeySchedule(mode_base, zz, info, default_psk, default_psk_id)
 
 let setupBaseR cs enc skR info =
   let pkR = DH.secret_to_public (curve_of_cs cs) skR in
-  let zz = decap cs enc skR in
-  match pkR, zz with
-  | Some pkR, Some zz ->
-    Some (key_schedule cs Base zz info None)
+  let shared_secret = decap cs enc skR in
+  match pkR, shared_secret with
+  | Some pkR, Some shared_secret ->
+    Some (key_schedule cs Base shared_secret info None)
   | _ -> None
 
 let sealBase cs skE pkR info aad pt =
@@ -454,41 +416,41 @@ let openBase cs enc skR info aad ct =
     | None -> None
     | Some (ctx, pt) -> Some pt
 
-/// def SetupPSKS(pkR, info, psk, pskID):
+/// def SetupPSKS(pkR, info, psk, psk_id):
 ///   zz, enc = Encap(pkR)
-///   return enc, KeySchedule(mode_psk, zz, info, psk, pskID)
+///   return enc, KeySchedule(mode_psk, zz, info, psk, psk_id)
 
-let setupPSKS cs skE pkR info psk pskID =
+let setupPSKS cs skE pkR info psk psk_id =
   match encap cs skE pkR with
   | None -> None
-  | Some (zz, enc) ->
-    assert (verify_psk_inputs cs PSK (Some (psk, pskID)));
-    let enc_ctx = key_schedule cs PSK zz info (Some (psk, pskID)) in
+  | Some (shared_secret, enc) ->
+    assert (verify_psk_inputs cs PSK (Some (psk, psk_id)));
+    let enc_ctx = key_schedule cs PSK shared_secret info (Some (psk, psk_id)) in
     Some (enc, enc_ctx)
 
 
-/// def SetupPSKR(enc, skR, info, psk, pskID):
+/// def SetupPSKR(enc, skR, info, psk, psk_id):
 ///   zz = Decap(enc, skR)
-///   return KeySchedule(mode_psk, zz, info, psk, pskID)
+///   return KeySchedule(mode_psk, zz, info, psk, psk_id)
 
-let setupPSKR cs enc skR info psk pskID =
+let setupPSKR cs enc skR info psk psk_id =
   let pkR = DH.secret_to_public (curve_of_cs cs) skR in
-  let zz = decap cs enc skR in
-  match pkR, zz with
-  | Some pkR, Some zz ->
-    Some (key_schedule cs PSK zz info (Some (psk, pskID)))
+  let shared_secret = decap cs enc skR in
+  match pkR, shared_secret with
+  | Some pkR, Some shared_secret ->
+    Some (key_schedule cs PSK shared_secret info (Some (psk, psk_id)))
   | _ -> None
 
-let sealPSK cs skE pkR info aad pt psk pskID =
-  match setupPSKS cs skE pkR info psk pskID with
+let sealPSK cs skE pkR info aad pt psk psk_id =
+  match setupPSKS cs skE pkR info psk psk_id with
   | None -> None
   | Some (enc, ctx) ->
     match context_seal cs ctx aad pt with
     | None -> None
     | Some (ctx, ct) -> Some (enc, ct)
 
-let openPSK cs enc skR info aad ct psk pskID =
-  match setupPSKR cs enc skR info psk pskID with
+let openPSK cs enc skR info aad ct psk psk_id =
+  match setupPSKR cs enc skR info psk psk_id with
   | None -> None
   | Some ctx ->
     match context_open cs ctx aad ct with
@@ -497,26 +459,26 @@ let openPSK cs enc skR info aad ct psk pskID =
 
 /// def SetupAuthS(pkR, info, skS):
 ///   zz, enc = AuthEncap(pkR, skS)
-///   return enc, KeySchedule(mode_auth, zz, info, default_psk, default_pskID)
+///   return enc, KeySchedule(mode_auth, zz, info, default_psk, default_psk_id)
 
 let setupAuthS cs skE pkR info skS =
   match auth_encap cs skE pkR skS with
   | None -> None
-  | Some (zz, enc) ->
-    let enc_ctx = key_schedule cs Auth zz info None in
+  | Some (shared_secret, enc) ->
+    let enc_ctx = key_schedule cs Auth shared_secret info None in
     Some (enc, enc_ctx)
 
 
 /// def SetupAuthR(enc, skR, info, pkS):
 ///   zz = AuthDecap(enc, skR, pkS)
-///   return KeySchedule(mode_auth, zz, info, default_psk, default_pskID)
+///   return KeySchedule(mode_auth, zz, info, default_psk, default_psk_id)
 
 let setupAuthR cs enc skR info pkS =
   let pkR = DH.secret_to_public (curve_of_cs cs) skR in
-  let zz = auth_decap cs enc skR pkS in
-  match pkR, zz with
-  | Some pkR, Some zz ->
-    Some (key_schedule cs Auth zz info None)
+  let shared_secret = auth_decap cs enc skR pkS in
+  match pkR, shared_secret with
+  | Some pkR, Some shared_secret ->
+    Some (key_schedule cs Auth shared_secret info None)
   | _ -> None
 
 let sealAuth cs skE pkR info aad pt skS =
@@ -535,43 +497,45 @@ let openAuth cs enc skR info aad ct pkS =
     | None -> None
     | Some (ctx, pt) -> Some pt
 
-/// def SetupAuthPSKS(pkR, info, psk, pskID, skS):
+/// def SetupAuthPSKS(pkR, info, psk, psk_id, skS):
 ///   zz, enc = AuthEncap(pkR, skS)
-///   return enc, KeySchedule(mode_auth_psk, zz, info, psk, pskID)
+///   return enc, KeySchedule(mode_auth_psk, zz, info, psk, psk_id)
 
-let setupAuthPSKS cs skE pkR info psk pskID skS =
+let setupAuthPSKS cs skE pkR info psk psk_id skS =
   match auth_encap cs skE pkR skS with
   | None -> None
-  | Some (zz, enc) ->
-    let enc_ctx = key_schedule cs AuthPSK zz info (Some (psk, pskID)) in
+  | Some (shared_secret, enc) ->
+    let enc_ctx = key_schedule cs AuthPSK shared_secret info (Some (psk, psk_id)) in
     Some (enc, enc_ctx)
 
 
-/// def SetupAuthPSKR(enc, skR, info, psk, pskID, pkS):
+/// def SetupAuthPSKR(enc, skR, info, psk, psk_id, pkS):
 ///   zz = AuthDecap(enc, skR, pkS)
-///   return KeySchedule(mode_auth_psk, zz, info, psk, pskID)
+///   return KeySchedule(mode_auth_psk, zz, info, psk, psk_id)
 
-let setupAuthPSKR cs enc skR info psk pskID pkS =
+let setupAuthPSKR cs enc skR info psk psk_id pkS =
   let pkR = DH.secret_to_public (curve_of_cs cs) skR in
-  let zz = auth_decap cs enc skR pkS in
-  match pkR, zz with
-  | Some pkR, Some zz ->
-    Some (key_schedule cs AuthPSK zz info (Some (psk, pskID)))
+  let shared_secret = auth_decap cs enc skR pkS in
+  match pkR, shared_secret with
+  | Some pkR, Some shared_secret ->
+    Some (key_schedule cs AuthPSK shared_secret info (Some (psk, psk_id)))
   | _ -> None
 
-let sealAuthPSK cs skE pkR info aad pt psk pskID skS =
-  match setupAuthPSKS cs skE pkR info psk pskID skS with
+let sealAuthPSK cs skE pkR info aad pt psk psk_id skS =
+  match setupAuthPSKS cs skE pkR info psk psk_id skS with
   | None -> None
   | Some (enc, ctx) ->
     match context_seal cs ctx aad pt with
     | None -> None
     | Some (ctx, ct) -> Some (enc, ct)
 
-let openAuthPSK cs enc skR info aad ct psk pskID pkS =
-  match setupAuthPSKR cs enc skR info psk pskID pkS with
+let openAuthPSK cs enc skR info aad ct psk psk_id pkS =
+  match setupAuthPSKR cs enc skR info psk psk_id pkS with
   | None -> None
   | Some ctx ->
     match context_open cs ctx aad ct with
     | None -> None
     | Some (ctx, pt) -> Some pt
 
+// TODO rename nonce to base_nonce
+// TODO single-shot export
