specs/tests/Spec.HPKE.Test.fst
@@ -56,7 +56,7 @@ let test_setupBase
   (enc0_nonce:HPKE.nonce_aead_s cs) (enc1_nonce:HPKE.nonce_aead_s cs)
 =
   print "Test setupBaseS\n";
-  let pkR = HPKE.unmarshal cs pkRm in
+  let pkR = HPKE.deserialize cs pkRm in
   match HPKE.setupBaseS cs skEm pkR info with
   | None -> false
   | Some (enc_i, ctx_i) -> print_and_compare_setup cs enc key nonce exp_sec enc_i ctx_i
@@ -86,15 +86,13 @@ let test_encryption
   print_and_compare_bytes (HPKE.size_aead_nonce cs) enc_nonce enc_nonce_i
 
 
-// Skipped unsupported test case 0
-
-let test1_mode: HPKE.mode = HPKE.Base
-let test1_ciphersuite = DH.DH_Curve25519, Hash.SHA2_256, AEAD.AES128_GCM, Hash.SHA2_256
+let test0_mode: HPKE.mode = HPKE.Base
+let test0_ciphersuite: HPKE.ciphersuite = DH.DH_Curve25519, Hash.SHA2_256, AEAD.AES128_GCM, Hash.SHA2_256
 
 // generated: "4f6465206f6e2061204772656369616e2055726e"
 inline_for_extraction
-let size_test1_info: size_nat = 20
-let test1_info_list : l:list uint8{List.Tot.length l == size_test1_info} =
+let size_test0_info: size_nat = 20
+let test0_info_list : l:list uint8{List.Tot.length l == size_test0_info} =
   [@inline_let]
   let l = [
     u8 0x4f; u8 0x64; u8 0x65; u8 0x20; u8 0x6f;
@@ -102,260 +100,294 @@ let test1_info_list : l:list uint8{List.Tot.length l == size_test1_info} =
     u8 0x72; u8 0x65; u8 0x63; u8 0x69; u8 0x61;
     u8 0x6e; u8 0x20; u8 0x55; u8 0x72; u8 0x6e;
   ] in
-  assert_norm(List.Tot.length l == size_test1_info);
+  assert_norm(List.Tot.length l == size_test0_info);
   l
-let test1_info : lbytes size_test1_info = createL test1_info_list
+let test0_info : lbytes size_test0_info = createL test0_info_list
 
-// generated: "919f0e1b7c361d1e5a3d0086ba94edeb6d2df9f756654741731f4e84cb813bdb"
+// generated: "6d9014e4609687b0a3670a22f2a14eac5ae6ad8c0beb62fb3ecb13dc8ebf5e06"
 inline_for_extraction
-let size_test1_skRm: size_nat = 32
-let test1_skRm_list : l:list uint8{List.Tot.length l == size_test1_skRm} =
+let size_test0_ikmR: size_nat = 32
+let test0_ikmR_list : l:list uint8{List.Tot.length l == size_test0_ikmR} =
   [@inline_let]
   let l = [
-    u8 0x91; u8 0x9f; u8 0x0e; u8 0x1b; u8 0x7c;
-    u8 0x36; u8 0x1d; u8 0x1e; u8 0x5a; u8 0x3d;
-    u8 0x00; u8 0x86; u8 0xba; u8 0x94; u8 0xed;
-    u8 0xeb; u8 0x6d; u8 0x2d; u8 0xf9; u8 0xf7;
-    u8 0x56; u8 0x65; u8 0x47; u8 0x41; u8 0x73;
-    u8 0x1f; u8 0x4e; u8 0x84; u8 0xcb; u8 0x81;
-    u8 0x3b; u8 0xdb;
+    u8 0x6d; u8 0x90; u8 0x14; u8 0xe4; u8 0x60;
+    u8 0x96; u8 0x87; u8 0xb0; u8 0xa3; u8 0x67;
+    u8 0x0a; u8 0x22; u8 0xf2; u8 0xa1; u8 0x4e;
+    u8 0xac; u8 0x5a; u8 0xe6; u8 0xad; u8 0x8c;
+    u8 0x0b; u8 0xeb; u8 0x62; u8 0xfb; u8 0x3e;
+    u8 0xcb; u8 0x13; u8 0xdc; u8 0x8e; u8 0xbf;
+    u8 0x5e; u8 0x06;
   ] in
-  assert_norm(List.Tot.length l == size_test1_skRm);
+  assert_norm(List.Tot.length l == size_test0_ikmR);
   l
-let test1_skRm : lbytes size_test1_skRm = createL test1_skRm_list
+let test0_ikmR : lbytes size_test0_ikmR = createL test0_ikmR_list
 
-// generated: "232ce0da9fd45b8d500781a5ee1b0a2cf64411dd08d6442400ab05a4d29733a8"
+// generated: "6305de86b3cec022fae6f2f2d2951f0f90c8662112124fd62f17e0a99bdbd08e"
 inline_for_extraction
-let size_test1_skEm: size_nat = 32
-let test1_skEm_list : l:list uint8{List.Tot.length l == size_test1_skEm} =
+let size_test0_ikmE: size_nat = 32
+let test0_ikmE_list : l:list uint8{List.Tot.length l == size_test0_ikmE} =
   [@inline_let]
   let l = [
-    u8 0x23; u8 0x2c; u8 0xe0; u8 0xda; u8 0x9f;
-    u8 0xd4; u8 0x5b; u8 0x8d; u8 0x50; u8 0x07;
-    u8 0x81; u8 0xa5; u8 0xee; u8 0x1b; u8 0x0a;
-    u8 0x2c; u8 0xf6; u8 0x44; u8 0x11; u8 0xdd;
-    u8 0x08; u8 0xd6; u8 0x44; u8 0x24; u8 0x00;
-    u8 0xab; u8 0x05; u8 0xa4; u8 0xd2; u8 0x97;
-    u8 0x33; u8 0xa8;
+    u8 0x63; u8 0x05; u8 0xde; u8 0x86; u8 0xb3;
+    u8 0xce; u8 0xc0; u8 0x22; u8 0xfa; u8 0xe6;
+    u8 0xf2; u8 0xf2; u8 0xd2; u8 0x95; u8 0x1f;
+    u8 0x0f; u8 0x90; u8 0xc8; u8 0x66; u8 0x21;
+    u8 0x12; u8 0x12; u8 0x4f; u8 0xd6; u8 0x2f;
+    u8 0x17; u8 0xe0; u8 0xa9; u8 0x9b; u8 0xdb;
+    u8 0xd0; u8 0x8e;
   ] in
-  assert_norm(List.Tot.length l == size_test1_skEm);
+  assert_norm(List.Tot.length l == size_test0_ikmE);
   l
-let test1_skEm : lbytes size_test1_skEm = createL test1_skEm_list
+let test0_ikmE : lbytes size_test0_ikmE = createL test0_ikmE_list
 
-// generated: "ac511615dee12b2e11170f1272c3972e6e2268d8fb05fc93c6b008065f61f22f"
+// generated: "ecaf25b8485bcf40b9f013dbb96a6230f25733b8435bba0997a1dedbc7f78806"
 inline_for_extraction
-let size_test1_pkRm: size_nat = 32
-let test1_pkRm_list : l:list uint8{List.Tot.length l == size_test1_pkRm} =
+let size_test0_skRm: size_nat = 32
+let test0_skRm_list : l:list uint8{List.Tot.length l == size_test0_skRm} =
   [@inline_let]
   let l = [
-    u8 0xac; u8 0x51; u8 0x16; u8 0x15; u8 0xde;
-    u8 0xe1; u8 0x2b; u8 0x2e; u8 0x11; u8 0x17;
-    u8 0x0f; u8 0x12; u8 0x72; u8 0xc3; u8 0x97;
-    u8 0x2e; u8 0x6e; u8 0x22; u8 0x68; u8 0xd8;
-    u8 0xfb; u8 0x05; u8 0xfc; u8 0x93; u8 0xc6;
-    u8 0xb0; u8 0x08; u8 0x06; u8 0x5f; u8 0x61;
-    u8 0xf2; u8 0x2f;
+    u8 0xec; u8 0xaf; u8 0x25; u8 0xb8; u8 0x48;
+    u8 0x5b; u8 0xcf; u8 0x40; u8 0xb9; u8 0xf0;
+    u8 0x13; u8 0xdb; u8 0xb9; u8 0x6a; u8 0x62;
+    u8 0x30; u8 0xf2; u8 0x57; u8 0x33; u8 0xb8;
+    u8 0x43; u8 0x5b; u8 0xba; u8 0x09; u8 0x97;
+    u8 0xa1; u8 0xde; u8 0xdb; u8 0xc7; u8 0xf7;
+    u8 0x88; u8 0x06;
   ] in
-  assert_norm(List.Tot.length l == size_test1_pkRm);
+  assert_norm(List.Tot.length l == size_test0_skRm);
   l
-let test1_pkRm : lbytes size_test1_pkRm = createL test1_pkRm_list
+let test0_skRm : lbytes size_test0_skRm = createL test0_skRm_list
 
-// generated: "ab8b7fdda7ed10c410079909350948ff63bc044b40575cc85636f3981bb8d258"
+// generated: "6cee2e2755790708a2a1be22667883a5e3f9ec52810404a0d889a0ed3e28de00"
 inline_for_extraction
-let size_test1_pkEm: size_nat = 32
-let test1_pkEm_list : l:list uint8{List.Tot.length l == size_test1_pkEm} =
+let size_test0_skEm: size_nat = 32
+let test0_skEm_list : l:list uint8{List.Tot.length l == size_test0_skEm} =
   [@inline_let]
   let l = [
-    u8 0xab; u8 0x8b; u8 0x7f; u8 0xdd; u8 0xa7;
-    u8 0xed; u8 0x10; u8 0xc4; u8 0x10; u8 0x07;
-    u8 0x99; u8 0x09; u8 0x35; u8 0x09; u8 0x48;
-    u8 0xff; u8 0x63; u8 0xbc; u8 0x04; u8 0x4b;
-    u8 0x40; u8 0x57; u8 0x5c; u8 0xc8; u8 0x56;
-    u8 0x36; u8 0xf3; u8 0x98; u8 0x1b; u8 0xb8;
-    u8 0xd2; u8 0x58;
+    u8 0x6c; u8 0xee; u8 0x2e; u8 0x27; u8 0x55;
+    u8 0x79; u8 0x07; u8 0x08; u8 0xa2; u8 0xa1;
+    u8 0xbe; u8 0x22; u8 0x66; u8 0x78; u8 0x83;
+    u8 0xa5; u8 0xe3; u8 0xf9; u8 0xec; u8 0x52;
+    u8 0x81; u8 0x04; u8 0x04; u8 0xa0; u8 0xd8;
+    u8 0x89; u8 0xa0; u8 0xed; u8 0x3e; u8 0x28;
+    u8 0xde; u8 0x00;
   ] in
-  assert_norm(List.Tot.length l == size_test1_pkEm);
+  assert_norm(List.Tot.length l == size_test0_skEm);
   l
-let test1_pkEm : lbytes size_test1_pkEm = createL test1_pkEm_list
+let test0_skEm : lbytes size_test0_skEm = createL test0_skEm_list
 
-// generated: "ab8b7fdda7ed10c410079909350948ff63bc044b40575cc85636f3981bb8d258"
+// generated: "a5912b20892e36905bac635267e2353d58f8cc7525271a2bf57b9c48d2ec2c07"
 inline_for_extraction
-let size_test1_enc: size_nat = 32
-let test1_enc_list : l:list uint8{List.Tot.length l == size_test1_enc} =
+let size_test0_pkRm: size_nat = 32
+let test0_pkRm_list : l:list uint8{List.Tot.length l == size_test0_pkRm} =
   [@inline_let]
   let l = [
-    u8 0xab; u8 0x8b; u8 0x7f; u8 0xdd; u8 0xa7;
-    u8 0xed; u8 0x10; u8 0xc4; u8 0x10; u8 0x07;
-    u8 0x99; u8 0x09; u8 0x35; u8 0x09; u8 0x48;
-    u8 0xff; u8 0x63; u8 0xbc; u8 0x04; u8 0x4b;
-    u8 0x40; u8 0x57; u8 0x5c; u8 0xc8; u8 0x56;
-    u8 0x36; u8 0xf3; u8 0x98; u8 0x1b; u8 0xb8;
-    u8 0xd2; u8 0x58;
+    u8 0xa5; u8 0x91; u8 0x2b; u8 0x20; u8 0x89;
+    u8 0x2e; u8 0x36; u8 0x90; u8 0x5b; u8 0xac;
+    u8 0x63; u8 0x52; u8 0x67; u8 0xe2; u8 0x35;
+    u8 0x3d; u8 0x58; u8 0xf8; u8 0xcc; u8 0x75;
+    u8 0x25; u8 0x27; u8 0x1a; u8 0x2b; u8 0xf5;
+    u8 0x7b; u8 0x9c; u8 0x48; u8 0xd2; u8 0xec;
+    u8 0x2c; u8 0x07;
   ] in
-  assert_norm(List.Tot.length l == size_test1_enc);
+  assert_norm(List.Tot.length l == size_test0_pkRm);
   l
-let test1_enc : lbytes size_test1_enc = createL test1_enc_list
+let test0_pkRm : lbytes size_test0_pkRm = createL test0_pkRm_list
 
-// generated: "44807c99177b0f3761d66f422945a21317a1532ca038e976594487a6a7e58fbf"
+// generated: "950897e0d37a8bdb0f2153edf5fa580a64b399c39fbb3d014f80983352a63617"
 inline_for_extraction
-let size_test1_zz: size_nat = 32
-let test1_zz_list : l:list uint8{List.Tot.length l == size_test1_zz} =
+let size_test0_pkEm: size_nat = 32
+let test0_pkEm_list : l:list uint8{List.Tot.length l == size_test0_pkEm} =
   [@inline_let]
   let l = [
-    u8 0x44; u8 0x80; u8 0x7c; u8 0x99; u8 0x17;
-    u8 0x7b; u8 0x0f; u8 0x37; u8 0x61; u8 0xd6;
-    u8 0x6f; u8 0x42; u8 0x29; u8 0x45; u8 0xa2;
-    u8 0x13; u8 0x17; u8 0xa1; u8 0x53; u8 0x2c;
-    u8 0xa0; u8 0x38; u8 0xe9; u8 0x76; u8 0x59;
-    u8 0x44; u8 0x87; u8 0xa6; u8 0xa7; u8 0xe5;
-    u8 0x8f; u8 0xbf;
+    u8 0x95; u8 0x08; u8 0x97; u8 0xe0; u8 0xd3;
+    u8 0x7a; u8 0x8b; u8 0xdb; u8 0x0f; u8 0x21;
+    u8 0x53; u8 0xed; u8 0xf5; u8 0xfa; u8 0x58;
+    u8 0x0a; u8 0x64; u8 0xb3; u8 0x99; u8 0xc3;
+    u8 0x9f; u8 0xbb; u8 0x3d; u8 0x01; u8 0x4f;
+    u8 0x80; u8 0x98; u8 0x33; u8 0x52; u8 0xa6;
+    u8 0x36; u8 0x17;
   ] in
-  assert_norm(List.Tot.length l == size_test1_zz);
+  assert_norm(List.Tot.length l == size_test0_pkEm);
   l
-let test1_zz : lbytes size_test1_zz = createL test1_zz_list
+let test0_pkEm : lbytes size_test0_pkEm = createL test0_pkEm_list
 
-// generated: "002000010001005d0f5548cb13d7eba5320ae0e21b1ee274aac7ea1cce02570cf993d1b2456449debcca602075cf6f8ef506613a82e1c73727e2c912d0c49f16cd56fc524af4ce"
+// generated: "950897e0d37a8bdb0f2153edf5fa580a64b399c39fbb3d014f80983352a63617"
 inline_for_extraction
-let size_test1_key_schedule_context: size_nat = 71
-let test1_key_schedule_context_list : l:list uint8{List.Tot.length l == size_test1_key_schedule_context} =
+let size_test0_enc: size_nat = 32
+let test0_enc_list : l:list uint8{List.Tot.length l == size_test0_enc} =
   [@inline_let]
   let l = [
-    u8 0x00; u8 0x20; u8 0x00; u8 0x01; u8 0x00;
-    u8 0x01; u8 0x00; u8 0x5d; u8 0x0f; u8 0x55;
-    u8 0x48; u8 0xcb; u8 0x13; u8 0xd7; u8 0xeb;
-    u8 0xa5; u8 0x32; u8 0x0a; u8 0xe0; u8 0xe2;
-    u8 0x1b; u8 0x1e; u8 0xe2; u8 0x74; u8 0xaa;
-    u8 0xc7; u8 0xea; u8 0x1c; u8 0xce; u8 0x02;
-    u8 0x57; u8 0x0c; u8 0xf9; u8 0x93; u8 0xd1;
-    u8 0xb2; u8 0x45; u8 0x64; u8 0x49; u8 0xde;
-    u8 0xbc; u8 0xca; u8 0x60; u8 0x20; u8 0x75;
-    u8 0xcf; u8 0x6f; u8 0x8e; u8 0xf5; u8 0x06;
-    u8 0x61; u8 0x3a; u8 0x82; u8 0xe1; u8 0xc7;
-    u8 0x37; u8 0x27; u8 0xe2; u8 0xc9; u8 0x12;
-    u8 0xd0; u8 0xc4; u8 0x9f; u8 0x16; u8 0xcd;
-    u8 0x56; u8 0xfc; u8 0x52; u8 0x4a; u8 0xf4;
-    u8 0xce;
+    u8 0x95; u8 0x08; u8 0x97; u8 0xe0; u8 0xd3;
+    u8 0x7a; u8 0x8b; u8 0xdb; u8 0x0f; u8 0x21;
+    u8 0x53; u8 0xed; u8 0xf5; u8 0xfa; u8 0x58;
+    u8 0x0a; u8 0x64; u8 0xb3; u8 0x99; u8 0xc3;
+    u8 0x9f; u8 0xbb; u8 0x3d; u8 0x01; u8 0x4f;
+    u8 0x80; u8 0x98; u8 0x33; u8 0x52; u8 0xa6;
+    u8 0x36; u8 0x17;
   ] in
-  assert_norm(List.Tot.length l == size_test1_key_schedule_context);
+  assert_norm(List.Tot.length l == size_test0_enc);
   l
-let test1_key_schedule_context : lbytes size_test1_key_schedule_context = createL test1_key_schedule_context_list
+let test0_enc : lbytes size_test0_enc = createL test0_enc_list
 
-// generated: "c104521df56de97b517165011f09e0ea2a36b9af339a9de402c8b88547c8b67e"
+// generated: "799b7b9a6a070e77ee9b9a2032f6624b273b532809c60200eba17ac3baf69a00"
 inline_for_extraction
-let size_test1_secret: size_nat = 32
-let test1_secret_list : l:list uint8{List.Tot.length l == size_test1_secret} =
+let size_test0_shared_secret: size_nat = 32
+let test0_shared_secret_list : l:list uint8{List.Tot.length l == size_test0_shared_secret} =
   [@inline_let]
   let l = [
-    u8 0xc1; u8 0x04; u8 0x52; u8 0x1d; u8 0xf5;
-    u8 0x6d; u8 0xe9; u8 0x7b; u8 0x51; u8 0x71;
-    u8 0x65; u8 0x01; u8 0x1f; u8 0x09; u8 0xe0;
-    u8 0xea; u8 0x2a; u8 0x36; u8 0xb9; u8 0xaf;
-    u8 0x33; u8 0x9a; u8 0x9d; u8 0xe4; u8 0x02;
-    u8 0xc8; u8 0xb8; u8 0x85; u8 0x47; u8 0xc8;
-    u8 0xb6; u8 0x7e;
+    u8 0x79; u8 0x9b; u8 0x7b; u8 0x9a; u8 0x6a;
+    u8 0x07; u8 0x0e; u8 0x77; u8 0xee; u8 0x9b;
+    u8 0x9a; u8 0x20; u8 0x32; u8 0xf6; u8 0x62;
+    u8 0x4b; u8 0x27; u8 0x3b; u8 0x53; u8 0x28;
+    u8 0x09; u8 0xc6; u8 0x02; u8 0x00; u8 0xeb;
+    u8 0xa1; u8 0x7a; u8 0xc3; u8 0xba; u8 0xf6;
+    u8 0x9a; u8 0x00;
   ] in
-  assert_norm(List.Tot.length l == size_test1_secret);
+  assert_norm(List.Tot.length l == size_test0_shared_secret);
   l
-let test1_secret : lbytes size_test1_secret = createL test1_secret_list
+let test0_shared_secret : lbytes size_test0_shared_secret = createL test0_shared_secret_list
 
-// generated: "e34afc8f8f4c2906b310d8e4e4d526f0"
+// generated: "002acc146c3ed28a930a50da2b269cb150a8a78a54081f81db457ac52d5bd2f581cb95a2c63b1dac72dc030fbe46d152ccb09f43fdf6e74d13660a4bd80ff49b55"
 inline_for_extraction
-let size_test1_key: size_nat = 16
-let test1_key_list : l:list uint8{List.Tot.length l == size_test1_key} =
+let size_test0_key_schedule_context: size_nat = 65
+let test0_key_schedule_context_list : l:list uint8{List.Tot.length l == size_test0_key_schedule_context} =
   [@inline_let]
   let l = [
-    u8 0xe3; u8 0x4a; u8 0xfc; u8 0x8f; u8 0x8f;
-    u8 0x4c; u8 0x29; u8 0x06; u8 0xb3; u8 0x10;
-    u8 0xd8; u8 0xe4; u8 0xe4; u8 0xd5; u8 0x26;
-    u8 0xf0;
+    u8 0x00; u8 0x2a; u8 0xcc; u8 0x14; u8 0x6c;
+    u8 0x3e; u8 0xd2; u8 0x8a; u8 0x93; u8 0x0a;
+    u8 0x50; u8 0xda; u8 0x2b; u8 0x26; u8 0x9c;
+    u8 0xb1; u8 0x50; u8 0xa8; u8 0xa7; u8 0x8a;
+    u8 0x54; u8 0x08; u8 0x1f; u8 0x81; u8 0xdb;
+    u8 0x45; u8 0x7a; u8 0xc5; u8 0x2d; u8 0x5b;
+    u8 0xd2; u8 0xf5; u8 0x81; u8 0xcb; u8 0x95;
+    u8 0xa2; u8 0xc6; u8 0x3b; u8 0x1d; u8 0xac;
+    u8 0x72; u8 0xdc; u8 0x03; u8 0x0f; u8 0xbe;
+    u8 0x46; u8 0xd1; u8 0x52; u8 0xcc; u8 0xb0;
+    u8 0x9f; u8 0x43; u8 0xfd; u8 0xf6; u8 0xe7;
+    u8 0x4d; u8 0x13; u8 0x66; u8 0x0a; u8 0x4b;
+    u8 0xd8; u8 0x0f; u8 0xf4; u8 0x9b; u8 0x55;
   ] in
-  assert_norm(List.Tot.length l == size_test1_key);
+  assert_norm(List.Tot.length l == size_test0_key_schedule_context);
   l
-let test1_key : lbytes size_test1_key = createL test1_key_list
+let test0_key_schedule_context : lbytes size_test0_key_schedule_context = createL test0_key_schedule_context_list
 
-// generated: "2764228860619e140920c7d7"
+// generated: "3ed37d4c4c7e3ebe6cb1fca03eabd4c878b442da340915d51d6ed49d8369d785"
 inline_for_extraction
-let size_test1_nonce: size_nat = 12
-let test1_nonce_list : l:list uint8{List.Tot.length l == size_test1_nonce} =
+let size_test0_secret: size_nat = 32
+let test0_secret_list : l:list uint8{List.Tot.length l == size_test0_secret} =
   [@inline_let]
   let l = [
-    u8 0x27; u8 0x64; u8 0x22; u8 0x88; u8 0x60;
-    u8 0x61; u8 0x9e; u8 0x14; u8 0x09; u8 0x20;
-    u8 0xc7; u8 0xd7;
+    u8 0x3e; u8 0xd3; u8 0x7d; u8 0x4c; u8 0x4c;
+    u8 0x7e; u8 0x3e; u8 0xbe; u8 0x6c; u8 0xb1;
+    u8 0xfc; u8 0xa0; u8 0x3e; u8 0xab; u8 0xd4;
+    u8 0xc8; u8 0x78; u8 0xb4; u8 0x42; u8 0xda;
+    u8 0x34; u8 0x09; u8 0x15; u8 0xd5; u8 0x1d;
+    u8 0x6e; u8 0xd4; u8 0x9d; u8 0x83; u8 0x69;
+    u8 0xd7; u8 0x85;
   ] in
-  assert_norm(List.Tot.length l == size_test1_nonce);
+  assert_norm(List.Tot.length l == size_test0_secret);
   l
-let test1_nonce : lbytes size_test1_nonce = createL test1_nonce_list
+let test0_secret : lbytes size_test0_secret = createL test0_secret_list
 
-// generated: "93c6a28ec7af55f669612d5d64fe680ae38ca88d14fb6ecba647606eee668124"
+// generated: "e20cee1bf5392ad2d3a442e231f187ae"
 inline_for_extraction
-let size_test1_exporterSecret: size_nat = 32
-let test1_exporterSecret_list : l:list uint8{List.Tot.length l == size_test1_exporterSecret} =
+let size_test0_key: size_nat = 16
+let test0_key_list : l:list uint8{List.Tot.length l == size_test0_key} =
   [@inline_let]
   let l = [
-    u8 0x93; u8 0xc6; u8 0xa2; u8 0x8e; u8 0xc7;
-    u8 0xaf; u8 0x55; u8 0xf6; u8 0x69; u8 0x61;
-    u8 0x2d; u8 0x5d; u8 0x64; u8 0xfe; u8 0x68;
-    u8 0x0a; u8 0xe3; u8 0x8c; u8 0xa8; u8 0x8d;
-    u8 0x14; u8 0xfb; u8 0x6e; u8 0xcb; u8 0xa6;
-    u8 0x47; u8 0x60; u8 0x6e; u8 0xee; u8 0x66;
-    u8 0x81; u8 0x24;
+    u8 0xe2; u8 0x0c; u8 0xee; u8 0x1b; u8 0xf5;
+    u8 0x39; u8 0x2a; u8 0xd2; u8 0xd3; u8 0xa4;
+    u8 0x42; u8 0xe2; u8 0x31; u8 0xf1; u8 0x87;
+    u8 0xae;
   ] in
-  assert_norm(List.Tot.length l == size_test1_exporterSecret);
+  assert_norm(List.Tot.length l == size_test0_key);
   l
-let test1_exporterSecret : lbytes size_test1_exporterSecret = createL test1_exporterSecret_list
+let test0_key : lbytes size_test0_key = createL test0_key_list
+
+// generated: "5d99b2f03c452f7a9441933a"
+inline_for_extraction
+let size_test0_base_nonce: size_nat = 12
+let test0_base_nonce_list : l:list uint8{List.Tot.length l == size_test0_base_nonce} =
+  [@inline_let]
+  let l = [
+    u8 0x5d; u8 0x99; u8 0xb2; u8 0xf0; u8 0x3c;
+    u8 0x45; u8 0x2f; u8 0x7a; u8 0x94; u8 0x41;
+    u8 0x93; u8 0x3a;
+  ] in
+  assert_norm(List.Tot.length l == size_test0_base_nonce);
+  l
+let test0_base_nonce : lbytes size_test0_base_nonce = createL test0_base_nonce_list
+
+// generated: "00c3cdacab28e981cc907d12e4f55f0aacae261dbb4eb610447a6bc431bfe2aa"
+inline_for_extraction
+let size_test0_exporter_secret: size_nat = 32
+let test0_exporter_secret_list : l:list uint8{List.Tot.length l == size_test0_exporter_secret} =
+  [@inline_let]
+  let l = [
+    u8 0x00; u8 0xc3; u8 0xcd; u8 0xac; u8 0xab;
+    u8 0x28; u8 0xe9; u8 0x81; u8 0xcc; u8 0x90;
+    u8 0x7d; u8 0x12; u8 0xe4; u8 0xf5; u8 0x5f;
+    u8 0x0a; u8 0xac; u8 0xae; u8 0x26; u8 0x1d;
+    u8 0xbb; u8 0x4e; u8 0xb6; u8 0x10; u8 0x44;
+    u8 0x7a; u8 0x6b; u8 0xc4; u8 0x31; u8 0xbf;
+    u8 0xe2; u8 0xaa;
+  ] in
+  assert_norm(List.Tot.length l == size_test0_exporter_secret);
+  l
+let test0_exporter_secret : lbytes size_test0_exporter_secret = createL test0_exporter_secret_list
 
 // generated: "436f756e742d30"
 inline_for_extraction
-let size_test1_encryption0_aad: size_nat = 7
-let test1_encryption0_aad_list : l:list uint8{List.Tot.length l == size_test1_encryption0_aad} =
+let size_test0_encryption0_aad: size_nat = 7
+let test0_encryption0_aad_list : l:list uint8{List.Tot.length l == size_test0_encryption0_aad} =
   [@inline_let]
   let l = [
     u8 0x43; u8 0x6f; u8 0x75; u8 0x6e; u8 0x74;
     u8 0x2d; u8 0x30;
   ] in
-  assert_norm(List.Tot.length l == size_test1_encryption0_aad);
+  assert_norm(List.Tot.length l == size_test0_encryption0_aad);
   l
-let test1_encryption0_aad : lbytes size_test1_encryption0_aad = createL test1_encryption0_aad_list
+let test0_encryption0_aad : lbytes size_test0_encryption0_aad = createL test0_encryption0_aad_list
 
-// generated: "1811cf5d39f857f80175f96ca4d3600bfb0585e4ce119bc46396da4b371966a358924e5a97a7b53ea255971f6b"
+// generated: "9418f1ae06eddc43aa911032aed4a951754ee2286a786733761857f8d96a7ec8d852da93bc5eeab49623344aba"
 inline_for_extraction
-let size_test1_encryption0_ciphertext: size_nat = 45
-let test1_encryption0_ciphertext_list : l:list uint8{List.Tot.length l == size_test1_encryption0_ciphertext} =
+let size_test0_encryption0_ciphertext: size_nat = 45
+let test0_encryption0_ciphertext_list : l:list uint8{List.Tot.length l == size_test0_encryption0_ciphertext} =
   [@inline_let]
   let l = [
-    u8 0x18; u8 0x11; u8 0xcf; u8 0x5d; u8 0x39;
-    u8 0xf8; u8 0x57; u8 0xf8; u8 0x01; u8 0x75;
-    u8 0xf9; u8 0x6c; u8 0xa4; u8 0xd3; u8 0x60;
-    u8 0x0b; u8 0xfb; u8 0x05; u8 0x85; u8 0xe4;
-    u8 0xce; u8 0x11; u8 0x9b; u8 0xc4; u8 0x63;
-    u8 0x96; u8 0xda; u8 0x4b; u8 0x37; u8 0x19;
-    u8 0x66; u8 0xa3; u8 0x58; u8 0x92; u8 0x4e;
-    u8 0x5a; u8 0x97; u8 0xa7; u8 0xb5; u8 0x3e;
-    u8 0xa2; u8 0x55; u8 0x97; u8 0x1f; u8 0x6b;
+    u8 0x94; u8 0x18; u8 0xf1; u8 0xae; u8 0x06;
+    u8 0xed; u8 0xdc; u8 0x43; u8 0xaa; u8 0x91;
+    u8 0x10; u8 0x32; u8 0xae; u8 0xd4; u8 0xa9;
+    u8 0x51; u8 0x75; u8 0x4e; u8 0xe2; u8 0x28;
+    u8 0x6a; u8 0x78; u8 0x67; u8 0x33; u8 0x76;
+    u8 0x18; u8 0x57; u8 0xf8; u8 0xd9; u8 0x6a;
+    u8 0x7e; u8 0xc8; u8 0xd8; u8 0x52; u8 0xda;
+    u8 0x93; u8 0xbc; u8 0x5e; u8 0xea; u8 0xb4;
+    u8 0x96; u8 0x23; u8 0x34; u8 0x4a; u8 0xba;
   ] in
-  assert_norm(List.Tot.length l == size_test1_encryption0_ciphertext);
+  assert_norm(List.Tot.length l == size_test0_encryption0_ciphertext);
   l
-let test1_encryption0_ciphertext : lbytes size_test1_encryption0_ciphertext = createL test1_encryption0_ciphertext_list
+let test0_encryption0_ciphertext : lbytes size_test0_encryption0_ciphertext = createL test0_encryption0_ciphertext_list
 
-// generated: "2764228860619e140920c7d7"
+// generated: "5d99b2f03c452f7a9441933a"
 inline_for_extraction
-let size_test1_encryption0_nonce: size_nat = 12
-let test1_encryption0_nonce_list : l:list uint8{List.Tot.length l == size_test1_encryption0_nonce} =
+let size_test0_encryption0_nonce: size_nat = 12
+let test0_encryption0_nonce_list : l:list uint8{List.Tot.length l == size_test0_encryption0_nonce} =
   [@inline_let]
   let l = [
-    u8 0x27; u8 0x64; u8 0x22; u8 0x88; u8 0x60;
-    u8 0x61; u8 0x9e; u8 0x14; u8 0x09; u8 0x20;
-    u8 0xc7; u8 0xd7;
+    u8 0x5d; u8 0x99; u8 0xb2; u8 0xf0; u8 0x3c;
+    u8 0x45; u8 0x2f; u8 0x7a; u8 0x94; u8 0x41;
+    u8 0x93; u8 0x3a;
   ] in
-  assert_norm(List.Tot.length l == size_test1_encryption0_nonce);
+  assert_norm(List.Tot.length l == size_test0_encryption0_nonce);
   l
-let test1_encryption0_nonce : lbytes size_test1_encryption0_nonce = createL test1_encryption0_nonce_list
+let test0_encryption0_nonce : lbytes size_test0_encryption0_nonce = createL test0_encryption0_nonce_list
 
 // generated: "4265617574792069732074727574682c20747275746820626561757479"
 inline_for_extraction
-let size_test1_encryption0_plaintext: size_nat = 29
-let test1_encryption0_plaintext_list : l:list uint8{List.Tot.length l == size_test1_encryption0_plaintext} =
+let size_test0_encryption0_plaintext: size_nat = 29
+let test0_encryption0_plaintext_list : l:list uint8{List.Tot.length l == size_test0_encryption0_plaintext} =
   [@inline_let]
   let l = [
     u8 0x42; u8 0x65; u8 0x61; u8 0x75; u8 0x74;
@@ -365,61 +397,61 @@ let test1_encryption0_plaintext_list : l:list uint8{List.Tot.length l == size_te
     u8 0x74; u8 0x68; u8 0x20; u8 0x62; u8 0x65;
     u8 0x61; u8 0x75; u8 0x74; u8 0x79;
   ] in
-  assert_norm(List.Tot.length l == size_test1_encryption0_plaintext);
+  assert_norm(List.Tot.length l == size_test0_encryption0_plaintext);
   l
-let test1_encryption0_plaintext : lbytes size_test1_encryption0_plaintext = createL test1_encryption0_plaintext_list
+let test0_encryption0_plaintext : lbytes size_test0_encryption0_plaintext = createL test0_encryption0_plaintext_list
 
 // generated: "436f756e742d31"
 inline_for_extraction
-let size_test1_encryption1_aad: size_nat = 7
-let test1_encryption1_aad_list : l:list uint8{List.Tot.length l == size_test1_encryption1_aad} =
+let size_test0_encryption1_aad: size_nat = 7
+let test0_encryption1_aad_list : l:list uint8{List.Tot.length l == size_test0_encryption1_aad} =
   [@inline_let]
   let l = [
     u8 0x43; u8 0x6f; u8 0x75; u8 0x6e; u8 0x74;
     u8 0x2d; u8 0x31;
   ] in
-  assert_norm(List.Tot.length l == size_test1_encryption1_aad);
+  assert_norm(List.Tot.length l == size_test0_encryption1_aad);
   l
-let test1_encryption1_aad : lbytes size_test1_encryption1_aad = createL test1_encryption1_aad_list
+let test0_encryption1_aad : lbytes size_test0_encryption1_aad = createL test0_encryption1_aad_list
 
-// generated: "2ed9ff66c33bad2f7c0326881f05aa9616ccba13bdb126a0d2a5a3dfa6b95bd4de78a98ff64c1fb64b366074d4"
+// generated: "74d69c61899b9158bb50e95d92fbad106f612ea67c61b3c4bef65c8bf3dc18e17bf41ec4c408688aae58358d0e"
 inline_for_extraction
-let size_test1_encryption1_ciphertext: size_nat = 45
-let test1_encryption1_ciphertext_list : l:list uint8{List.Tot.length l == size_test1_encryption1_ciphertext} =
+let size_test0_encryption1_ciphertext: size_nat = 45
+let test0_encryption1_ciphertext_list : l:list uint8{List.Tot.length l == size_test0_encryption1_ciphertext} =
   [@inline_let]
   let l = [
-    u8 0x2e; u8 0xd9; u8 0xff; u8 0x66; u8 0xc3;
-    u8 0x3b; u8 0xad; u8 0x2f; u8 0x7c; u8 0x03;
-    u8 0x26; u8 0x88; u8 0x1f; u8 0x05; u8 0xaa;
-    u8 0x96; u8 0x16; u8 0xcc; u8 0xba; u8 0x13;
-    u8 0xbd; u8 0xb1; u8 0x26; u8 0xa0; u8 0xd2;
-    u8 0xa5; u8 0xa3; u8 0xdf; u8 0xa6; u8 0xb9;
-    u8 0x5b; u8 0xd4; u8 0xde; u8 0x78; u8 0xa9;
-    u8 0x8f; u8 0xf6; u8 0x4c; u8 0x1f; u8 0xb6;
-    u8 0x4b; u8 0x36; u8 0x60; u8 0x74; u8 0xd4;
+    u8 0x74; u8 0xd6; u8 0x9c; u8 0x61; u8 0x89;
+    u8 0x9b; u8 0x91; u8 0x58; u8 0xbb; u8 0x50;
+    u8 0xe9; u8 0x5d; u8 0x92; u8 0xfb; u8 0xad;
+    u8 0x10; u8 0x6f; u8 0x61; u8 0x2e; u8 0xa6;
+    u8 0x7c; u8 0x61; u8 0xb3; u8 0xc4; u8 0xbe;
+    u8 0xf6; u8 0x5c; u8 0x8b; u8 0xf3; u8 0xdc;
+    u8 0x18; u8 0xe1; u8 0x7b; u8 0xf4; u8 0x1e;
+    u8 0xc4; u8 0xc4; u8 0x08; u8 0x68; u8 0x8a;
+    u8 0xae; u8 0x58; u8 0x35; u8 0x8d; u8 0x0e;
   ] in
-  assert_norm(List.Tot.length l == size_test1_encryption1_ciphertext);
+  assert_norm(List.Tot.length l == size_test0_encryption1_ciphertext);
   l
-let test1_encryption1_ciphertext : lbytes size_test1_encryption1_ciphertext = createL test1_encryption1_ciphertext_list
+let test0_encryption1_ciphertext : lbytes size_test0_encryption1_ciphertext = createL test0_encryption1_ciphertext_list
 
-// generated: "2764228860619e140920c7d6"
+// generated: "5d99b2f03c452f7a9441933b"
 inline_for_extraction
-let size_test1_encryption1_nonce: size_nat = 12
-let test1_encryption1_nonce_list : l:list uint8{List.Tot.length l == size_test1_encryption1_nonce} =
+let size_test0_encryption1_nonce: size_nat = 12
+let test0_encryption1_nonce_list : l:list uint8{List.Tot.length l == size_test0_encryption1_nonce} =
   [@inline_let]
   let l = [
-    u8 0x27; u8 0x64; u8 0x22; u8 0x88; u8 0x60;
-    u8 0x61; u8 0x9e; u8 0x14; u8 0x09; u8 0x20;
-    u8 0xc7; u8 0xd6;
+    u8 0x5d; u8 0x99; u8 0xb2; u8 0xf0; u8 0x3c;
+    u8 0x45; u8 0x2f; u8 0x7a; u8 0x94; u8 0x41;
+    u8 0x93; u8 0x3b;
   ] in
-  assert_norm(List.Tot.length l == size_test1_encryption1_nonce);
+  assert_norm(List.Tot.length l == size_test0_encryption1_nonce);
   l
-let test1_encryption1_nonce : lbytes size_test1_encryption1_nonce = createL test1_encryption1_nonce_list
+let test0_encryption1_nonce : lbytes size_test0_encryption1_nonce = createL test0_encryption1_nonce_list
 
 // generated: "4265617574792069732074727574682c20747275746820626561757479"
 inline_for_extraction
-let size_test1_encryption1_plaintext: size_nat = 29
-let test1_encryption1_plaintext_list : l:list uint8{List.Tot.length l == size_test1_encryption1_plaintext} =
+let size_test0_encryption1_plaintext: size_nat = 29
+let test0_encryption1_plaintext_list : l:list uint8{List.Tot.length l == size_test0_encryption1_plaintext} =
   [@inline_let]
   let l = [
     u8 0x42; u8 0x65; u8 0x61; u8 0x75; u8 0x74;
@@ -429,735 +461,89 @@ let test1_encryption1_plaintext_list : l:list uint8{List.Tot.length l == size_te
     u8 0x74; u8 0x68; u8 0x20; u8 0x62; u8 0x65;
     u8 0x61; u8 0x75; u8 0x74; u8 0x79;
   ] in
-  assert_norm(List.Tot.length l == size_test1_encryption1_plaintext);
+  assert_norm(List.Tot.length l == size_test0_encryption1_plaintext);
   l
-let test1_encryption1_plaintext : lbytes size_test1_encryption1_plaintext = createL test1_encryption1_plaintext_list
-
-// generated: "436f756e742d32"
+let test0_encryption1_plaintext : lbytes size_test0_encryption1_plaintext = createL test0_encryption1_plaintext_list
+// generated: ""
 inline_for_extraction
-let size_test1_encryption2_aad: size_nat = 7
-let test1_encryption2_aad_list : l:list uint8{List.Tot.length l == size_test1_encryption2_aad} =
+let size_test0_export0_exporter_context: size_nat = 0
+let test0_export0_exporter_context_list : l:list uint8{List.Tot.length l == size_test0_export0_exporter_context} =
   [@inline_let]
   let l = [
-    u8 0x43; u8 0x6f; u8 0x75; u8 0x6e; u8 0x74;
-    u8 0x2d; u8 0x32;
-  ] in
-  assert_norm(List.Tot.length l == size_test1_encryption2_aad);
-  l
-let test1_encryption2_aad : lbytes size_test1_encryption2_aad = createL test1_encryption2_aad_list
 
-// generated: "4bfc8da6f1da808be2c1c141e864fe536bd1e9c4e01376cd383370b8095438a06f372e663739b30af9355da8a3"
+  ] in
+  assert_norm(List.Tot.length l == size_test0_export0_exporter_context);
+  l
+let test0_export0_exporter_context : lbytes size_test0_export0_exporter_context = createL test0_export0_exporter_context_list
+
+// generated: "be82c06bd83fd6edd74385de5a70859b9e03def4c7bb224a10cfae86087f8a25"
 inline_for_extraction
-let size_test1_encryption2_ciphertext: size_nat = 45
-let test1_encryption2_ciphertext_list : l:list uint8{List.Tot.length l == size_test1_encryption2_ciphertext} =
+let size_test0_export0_exported_value: size_nat = 32
+let test0_export0_exported_value_list : l:list uint8{List.Tot.length l == size_test0_export0_exported_value} =
   [@inline_let]
   let l = [
-    u8 0x4b; u8 0xfc; u8 0x8d; u8 0xa6; u8 0xf1;
-    u8 0xda; u8 0x80; u8 0x8b; u8 0xe2; u8 0xc1;
-    u8 0xc1; u8 0x41; u8 0xe8; u8 0x64; u8 0xfe;
-    u8 0x53; u8 0x6b; u8 0xd1; u8 0xe9; u8 0xc4;
-    u8 0xe0; u8 0x13; u8 0x76; u8 0xcd; u8 0x38;
-    u8 0x33; u8 0x70; u8 0xb8; u8 0x09; u8 0x54;
-    u8 0x38; u8 0xa0; u8 0x6f; u8 0x37; u8 0x2e;
-    u8 0x66; u8 0x37; u8 0x39; u8 0xb3; u8 0x0a;
-    u8 0xf9; u8 0x35; u8 0x5d; u8 0xa8; u8 0xa3;
+    u8 0xbe; u8 0x82; u8 0xc0; u8 0x6b; u8 0xd8;
+    u8 0x3f; u8 0xd6; u8 0xed; u8 0xd7; u8 0x43;
+    u8 0x85; u8 0xde; u8 0x5a; u8 0x70; u8 0x85;
+    u8 0x9b; u8 0x9e; u8 0x03; u8 0xde; u8 0xf4;
+    u8 0xc7; u8 0xbb; u8 0x22; u8 0x4a; u8 0x10;
+    u8 0xcf; u8 0xae; u8 0x86; u8 0x08; u8 0x7f;
+    u8 0x8a; u8 0x25;
   ] in
-  assert_norm(List.Tot.length l == size_test1_encryption2_ciphertext);
+  assert_norm(List.Tot.length l == size_test0_export0_exported_value);
   l
-let test1_encryption2_ciphertext : lbytes size_test1_encryption2_ciphertext = createL test1_encryption2_ciphertext_list
+let test0_export0_exported_value : lbytes size_test0_export0_exported_value = createL test0_export0_exported_value_list
 
-// generated: "2764228860619e140920c7d5"
+let test0_export0_len:size_nat = 32
+// generated: "00"
 inline_for_extraction
-let size_test1_encryption2_nonce: size_nat = 12
-let test1_encryption2_nonce_list : l:list uint8{List.Tot.length l == size_test1_encryption2_nonce} =
+let size_test0_export1_exporter_context: size_nat = 1
+let test0_export1_exporter_context_list : l:list uint8{List.Tot.length l == size_test0_export1_exporter_context} =
   [@inline_let]
   let l = [
-    u8 0x27; u8 0x64; u8 0x22; u8 0x88; u8 0x60;
-    u8 0x61; u8 0x9e; u8 0x14; u8 0x09; u8 0x20;
-    u8 0xc7; u8 0xd5;
+    u8 0x00;
   ] in
-  assert_norm(List.Tot.length l == size_test1_encryption2_nonce);
+  assert_norm(List.Tot.length l == size_test0_export1_exporter_context);
   l
-let test1_encryption2_nonce : lbytes size_test1_encryption2_nonce = createL test1_encryption2_nonce_list
+let test0_export1_exporter_context : lbytes size_test0_export1_exporter_context = createL test0_export1_exporter_context_list
 
-// generated: "4265617574792069732074727574682c20747275746820626561757479"
+// generated: "82cbfd3c2b2db75e2311d457e569cf12b6387eb4309bca8e77adb2f2b599fc85"
 inline_for_extraction
-let size_test1_encryption2_plaintext: size_nat = 29
-let test1_encryption2_plaintext_list : l:list uint8{List.Tot.length l == size_test1_encryption2_plaintext} =
+let size_test0_export1_exported_value: size_nat = 32
+let test0_export1_exported_value_list : l:list uint8{List.Tot.length l == size_test0_export1_exported_value} =
   [@inline_let]
   let l = [
-    u8 0x42; u8 0x65; u8 0x61; u8 0x75; u8 0x74;
-    u8 0x79; u8 0x20; u8 0x69; u8 0x73; u8 0x20;
-    u8 0x74; u8 0x72; u8 0x75; u8 0x74; u8 0x68;
-    u8 0x2c; u8 0x20; u8 0x74; u8 0x72; u8 0x75;
-    u8 0x74; u8 0x68; u8 0x20; u8 0x62; u8 0x65;
-    u8 0x61; u8 0x75; u8 0x74; u8 0x79;
+    u8 0x82; u8 0xcb; u8 0xfd; u8 0x3c; u8 0x2b;
+    u8 0x2d; u8 0xb7; u8 0x5e; u8 0x23; u8 0x11;
+    u8 0xd4; u8 0x57; u8 0xe5; u8 0x69; u8 0xcf;
+    u8 0x12; u8 0xb6; u8 0x38; u8 0x7e; u8 0xb4;
+    u8 0x30; u8 0x9b; u8 0xca; u8 0x8e; u8 0x77;
+    u8 0xad; u8 0xb2; u8 0xf2; u8 0xb5; u8 0x99;
+    u8 0xfc; u8 0x85;
   ] in
-  assert_norm(List.Tot.length l == size_test1_encryption2_plaintext);
+  assert_norm(List.Tot.length l == size_test0_export1_exported_value);
   l
-let test1_encryption2_plaintext : lbytes size_test1_encryption2_plaintext = createL test1_encryption2_plaintext_list
+let test0_export1_exported_value : lbytes size_test0_export1_exported_value = createL test0_export1_exported_value_list
 
-// generated: "436f756e742d33"
-inline_for_extraction
-let size_test1_encryption3_aad: size_nat = 7
-let test1_encryption3_aad_list : l:list uint8{List.Tot.length l == size_test1_encryption3_aad} =
-  [@inline_let]
-  let l = [
-    u8 0x43; u8 0x6f; u8 0x75; u8 0x6e; u8 0x74;
-    u8 0x2d; u8 0x33;
-  ] in
-  assert_norm(List.Tot.length l == size_test1_encryption3_aad);
-  l
-let test1_encryption3_aad : lbytes size_test1_encryption3_aad = createL test1_encryption3_aad_list
+let test0_export1_len:size_nat = 32
 
-// generated: "cc82487c2beb92d6810a40bad2aa96794c5f2b6eff96a674cf9c9c853397e6c7ca9640c200a38326adb63ed7f2"
-inline_for_extraction
-let size_test1_encryption3_ciphertext: size_nat = 45
-let test1_encryption3_ciphertext_list : l:list uint8{List.Tot.length l == size_test1_encryption3_ciphertext} =
-  [@inline_let]
-  let l = [
-    u8 0xcc; u8 0x82; u8 0x48; u8 0x7c; u8 0x2b;
-    u8 0xeb; u8 0x92; u8 0xd6; u8 0x81; u8 0x0a;
-    u8 0x40; u8 0xba; u8 0xd2; u8 0xaa; u8 0x96;
-    u8 0x79; u8 0x4c; u8 0x5f; u8 0x2b; u8 0x6e;
-    u8 0xff; u8 0x96; u8 0xa6; u8 0x74; u8 0xcf;
-    u8 0x9c; u8 0x9c; u8 0x85; u8 0x33; u8 0x97;
-    u8 0xe6; u8 0xc7; u8 0xca; u8 0x96; u8 0x40;
-    u8 0xc2; u8 0x00; u8 0xa3; u8 0x83; u8 0x26;
-    u8 0xad; u8 0xb6; u8 0x3e; u8 0xd7; u8 0xf2;
-  ] in
-  assert_norm(List.Tot.length l == size_test1_encryption3_ciphertext);
-  l
-let test1_encryption3_ciphertext : lbytes size_test1_encryption3_ciphertext = createL test1_encryption3_ciphertext_list
 
-// generated: "2764228860619e140920c7d4"
-inline_for_extraction
-let size_test1_encryption3_nonce: size_nat = 12
-let test1_encryption3_nonce_list : l:list uint8{List.Tot.length l == size_test1_encryption3_nonce} =
-  [@inline_let]
-  let l = [
-    u8 0x27; u8 0x64; u8 0x22; u8 0x88; u8 0x60;
-    u8 0x61; u8 0x9e; u8 0x14; u8 0x09; u8 0x20;
-    u8 0xc7; u8 0xd4;
-  ] in
-  assert_norm(List.Tot.length l == size_test1_encryption3_nonce);
-  l
-let test1_encryption3_nonce : lbytes size_test1_encryption3_nonce = createL test1_encryption3_nonce_list
-
-// generated: "4265617574792069732074727574682c20747275746820626561757479"
-inline_for_extraction
-let size_test1_encryption3_plaintext: size_nat = 29
-let test1_encryption3_plaintext_list : l:list uint8{List.Tot.length l == size_test1_encryption3_plaintext} =
-  [@inline_let]
-  let l = [
-    u8 0x42; u8 0x65; u8 0x61; u8 0x75; u8 0x74;
-    u8 0x79; u8 0x20; u8 0x69; u8 0x73; u8 0x20;
-    u8 0x74; u8 0x72; u8 0x75; u8 0x74; u8 0x68;
-    u8 0x2c; u8 0x20; u8 0x74; u8 0x72; u8 0x75;
-    u8 0x74; u8 0x68; u8 0x20; u8 0x62; u8 0x65;
-    u8 0x61; u8 0x75; u8 0x74; u8 0x79;
-  ] in
-  assert_norm(List.Tot.length l == size_test1_encryption3_plaintext);
-  l
-let test1_encryption3_plaintext : lbytes size_test1_encryption3_plaintext = createL test1_encryption3_plaintext_list
-
-// generated: "436f756e742d34"
-inline_for_extraction
-let size_test1_encryption4_aad: size_nat = 7
-let test1_encryption4_aad_list : l:list uint8{List.Tot.length l == size_test1_encryption4_aad} =
-  [@inline_let]
-  let l = [
-    u8 0x43; u8 0x6f; u8 0x75; u8 0x6e; u8 0x74;
-    u8 0x2d; u8 0x34;
-  ] in
-  assert_norm(List.Tot.length l == size_test1_encryption4_aad);
-  l
-let test1_encryption4_aad : lbytes size_test1_encryption4_aad = createL test1_encryption4_aad_list
-
-// generated: "6314e60548cfdc30552303be4cb19875e335554bce186e1b41f9d15b4b4a4af77d68c09ebf883a9cbb51f3be9d"
-inline_for_extraction
-let size_test1_encryption4_ciphertext: size_nat = 45
-let test1_encryption4_ciphertext_list : l:list uint8{List.Tot.length l == size_test1_encryption4_ciphertext} =
-  [@inline_let]
-  let l = [
-    u8 0x63; u8 0x14; u8 0xe6; u8 0x05; u8 0x48;
-    u8 0xcf; u8 0xdc; u8 0x30; u8 0x55; u8 0x23;
-    u8 0x03; u8 0xbe; u8 0x4c; u8 0xb1; u8 0x98;
-    u8 0x75; u8 0xe3; u8 0x35; u8 0x55; u8 0x4b;
-    u8 0xce; u8 0x18; u8 0x6e; u8 0x1b; u8 0x41;
-    u8 0xf9; u8 0xd1; u8 0x5b; u8 0x4b; u8 0x4a;
-    u8 0x4a; u8 0xf7; u8 0x7d; u8 0x68; u8 0xc0;
-    u8 0x9e; u8 0xbf; u8 0x88; u8 0x3a; u8 0x9c;
-    u8 0xbb; u8 0x51; u8 0xf3; u8 0xbe; u8 0x9d;
-  ] in
-  assert_norm(List.Tot.length l == size_test1_encryption4_ciphertext);
-  l
-let test1_encryption4_ciphertext : lbytes size_test1_encryption4_ciphertext = createL test1_encryption4_ciphertext_list
-
-// generated: "2764228860619e140920c7d3"
-inline_for_extraction
-let size_test1_encryption4_nonce: size_nat = 12
-let test1_encryption4_nonce_list : l:list uint8{List.Tot.length l == size_test1_encryption4_nonce} =
-  [@inline_let]
-  let l = [
-    u8 0x27; u8 0x64; u8 0x22; u8 0x88; u8 0x60;
-    u8 0x61; u8 0x9e; u8 0x14; u8 0x09; u8 0x20;
-    u8 0xc7; u8 0xd3;
-  ] in
-  assert_norm(List.Tot.length l == size_test1_encryption4_nonce);
-  l
-let test1_encryption4_nonce : lbytes size_test1_encryption4_nonce = createL test1_encryption4_nonce_list
-
-// generated: "4265617574792069732074727574682c20747275746820626561757479"
-inline_for_extraction
-let size_test1_encryption4_plaintext: size_nat = 29
-let test1_encryption4_plaintext_list : l:list uint8{List.Tot.length l == size_test1_encryption4_plaintext} =
-  [@inline_let]
-  let l = [
-    u8 0x42; u8 0x65; u8 0x61; u8 0x75; u8 0x74;
-    u8 0x79; u8 0x20; u8 0x69; u8 0x73; u8 0x20;
-    u8 0x74; u8 0x72; u8 0x75; u8 0x74; u8 0x68;
-    u8 0x2c; u8 0x20; u8 0x74; u8 0x72; u8 0x75;
-    u8 0x74; u8 0x68; u8 0x20; u8 0x62; u8 0x65;
-    u8 0x61; u8 0x75; u8 0x74; u8 0x79;
-  ] in
-  assert_norm(List.Tot.length l == size_test1_encryption4_plaintext);
-  l
-let test1_encryption4_plaintext : lbytes size_test1_encryption4_plaintext = createL test1_encryption4_plaintext_list
-
-// generated: "436f756e742d35"
-inline_for_extraction
-let size_test1_encryption5_aad: size_nat = 7
-let test1_encryption5_aad_list : l:list uint8{List.Tot.length l == size_test1_encryption5_aad} =
-  [@inline_let]
-  let l = [
-    u8 0x43; u8 0x6f; u8 0x75; u8 0x6e; u8 0x74;
-    u8 0x2d; u8 0x35;
-  ] in
-  assert_norm(List.Tot.length l == size_test1_encryption5_aad);
-  l
-let test1_encryption5_aad : lbytes size_test1_encryption5_aad = createL test1_encryption5_aad_list
-
-// generated: "ce580d139c001ed794c4eedf14ce43c19c2a04f20dcfa9de57b6f555816b0558db4ec603bbc3748dce30e5c82f"
-inline_for_extraction
-let size_test1_encryption5_ciphertext: size_nat = 45
-let test1_encryption5_ciphertext_list : l:list uint8{List.Tot.length l == size_test1_encryption5_ciphertext} =
-  [@inline_let]
-  let l = [
-    u8 0xce; u8 0x58; u8 0x0d; u8 0x13; u8 0x9c;
-    u8 0x00; u8 0x1e; u8 0xd7; u8 0x94; u8 0xc4;
-    u8 0xee; u8 0xdf; u8 0x14; u8 0xce; u8 0x43;
-    u8 0xc1; u8 0x9c; u8 0x2a; u8 0x04; u8 0xf2;
-    u8 0x0d; u8 0xcf; u8 0xa9; u8 0xde; u8 0x57;
-    u8 0xb6; u8 0xf5; u8 0x55; u8 0x81; u8 0x6b;
-    u8 0x05; u8 0x58; u8 0xdb; u8 0x4e; u8 0xc6;
-    u8 0x03; u8 0xbb; u8 0xc3; u8 0x74; u8 0x8d;
-    u8 0xce; u8 0x30; u8 0xe5; u8 0xc8; u8 0x2f;
-  ] in
-  assert_norm(List.Tot.length l == size_test1_encryption5_ciphertext);
-  l
-let test1_encryption5_ciphertext : lbytes size_test1_encryption5_ciphertext = createL test1_encryption5_ciphertext_list
-
-// generated: "2764228860619e140920c7d2"
-inline_for_extraction
-let size_test1_encryption5_nonce: size_nat = 12
-let test1_encryption5_nonce_list : l:list uint8{List.Tot.length l == size_test1_encryption5_nonce} =
-  [@inline_let]
-  let l = [
-    u8 0x27; u8 0x64; u8 0x22; u8 0x88; u8 0x60;
-    u8 0x61; u8 0x9e; u8 0x14; u8 0x09; u8 0x20;
-    u8 0xc7; u8 0xd2;
-  ] in
-  assert_norm(List.Tot.length l == size_test1_encryption5_nonce);
-  l
-let test1_encryption5_nonce : lbytes size_test1_encryption5_nonce = createL test1_encryption5_nonce_list
-
-// generated: "4265617574792069732074727574682c20747275746820626561757479"
-inline_for_extraction
-let size_test1_encryption5_plaintext: size_nat = 29
-let test1_encryption5_plaintext_list : l:list uint8{List.Tot.length l == size_test1_encryption5_plaintext} =
-  [@inline_let]
-  let l = [
-    u8 0x42; u8 0x65; u8 0x61; u8 0x75; u8 0x74;
-    u8 0x79; u8 0x20; u8 0x69; u8 0x73; u8 0x20;
-    u8 0x74; u8 0x72; u8 0x75; u8 0x74; u8 0x68;
-    u8 0x2c; u8 0x20; u8 0x74; u8 0x72; u8 0x75;
-    u8 0x74; u8 0x68; u8 0x20; u8 0x62; u8 0x65;
-    u8 0x61; u8 0x75; u8 0x74; u8 0x79;
-  ] in
-  assert_norm(List.Tot.length l == size_test1_encryption5_plaintext);
-  l
-let test1_encryption5_plaintext : lbytes size_test1_encryption5_plaintext = createL test1_encryption5_plaintext_list
-
-// generated: "436f756e742d36"
-inline_for_extraction
-let size_test1_encryption6_aad: size_nat = 7
-let test1_encryption6_aad_list : l:list uint8{List.Tot.length l == size_test1_encryption6_aad} =
-  [@inline_let]
-  let l = [
-    u8 0x43; u8 0x6f; u8 0x75; u8 0x6e; u8 0x74;
-    u8 0x2d; u8 0x36;
-  ] in
-  assert_norm(List.Tot.length l == size_test1_encryption6_aad);
-  l
-let test1_encryption6_aad : lbytes size_test1_encryption6_aad = createL test1_encryption6_aad_list
-
-// generated: "5247db08759b2a6d9459a4cc461dfc59afb78e37b0852f9a669720df72fe5781460bcc9ae5ca00545ad06f93c3"
-inline_for_extraction
-let size_test1_encryption6_ciphertext: size_nat = 45
-let test1_encryption6_ciphertext_list : l:list uint8{List.Tot.length l == size_test1_encryption6_ciphertext} =
-  [@inline_let]
-  let l = [
-    u8 0x52; u8 0x47; u8 0xdb; u8 0x08; u8 0x75;
-    u8 0x9b; u8 0x2a; u8 0x6d; u8 0x94; u8 0x59;
-    u8 0xa4; u8 0xcc; u8 0x46; u8 0x1d; u8 0xfc;
-    u8 0x59; u8 0xaf; u8 0xb7; u8 0x8e; u8 0x37;
-    u8 0xb0; u8 0x85; u8 0x2f; u8 0x9a; u8 0x66;
-    u8 0x97; u8 0x20; u8 0xdf; u8 0x72; u8 0xfe;
-    u8 0x57; u8 0x81; u8 0x46; u8 0x0b; u8 0xcc;
-    u8 0x9a; u8 0xe5; u8 0xca; u8 0x00; u8 0x54;
-    u8 0x5a; u8 0xd0; u8 0x6f; u8 0x93; u8 0xc3;
-  ] in
-  assert_norm(List.Tot.length l == size_test1_encryption6_ciphertext);
-  l
-let test1_encryption6_ciphertext : lbytes size_test1_encryption6_ciphertext = createL test1_encryption6_ciphertext_list
-
-// generated: "2764228860619e140920c7d1"
-inline_for_extraction
-let size_test1_encryption6_nonce: size_nat = 12
-let test1_encryption6_nonce_list : l:list uint8{List.Tot.length l == size_test1_encryption6_nonce} =
-  [@inline_let]
-  let l = [
-    u8 0x27; u8 0x64; u8 0x22; u8 0x88; u8 0x60;
-    u8 0x61; u8 0x9e; u8 0x14; u8 0x09; u8 0x20;
-    u8 0xc7; u8 0xd1;
-  ] in
-  assert_norm(List.Tot.length l == size_test1_encryption6_nonce);
-  l
-let test1_encryption6_nonce : lbytes size_test1_encryption6_nonce = createL test1_encryption6_nonce_list
-
-// generated: "4265617574792069732074727574682c20747275746820626561757479"
-inline_for_extraction
-let size_test1_encryption6_plaintext: size_nat = 29
-let test1_encryption6_plaintext_list : l:list uint8{List.Tot.length l == size_test1_encryption6_plaintext} =
-  [@inline_let]
-  let l = [
-    u8 0x42; u8 0x65; u8 0x61; u8 0x75; u8 0x74;
-    u8 0x79; u8 0x20; u8 0x69; u8 0x73; u8 0x20;
-    u8 0x74; u8 0x72; u8 0x75; u8 0x74; u8 0x68;
-    u8 0x2c; u8 0x20; u8 0x74; u8 0x72; u8 0x75;
-    u8 0x74; u8 0x68; u8 0x20; u8 0x62; u8 0x65;
-    u8 0x61; u8 0x75; u8 0x74; u8 0x79;
-  ] in
-  assert_norm(List.Tot.length l == size_test1_encryption6_plaintext);
-  l
-let test1_encryption6_plaintext : lbytes size_test1_encryption6_plaintext = createL test1_encryption6_plaintext_list
-
-// generated: "436f756e742d37"
-inline_for_extraction
-let size_test1_encryption7_aad: size_nat = 7
-let test1_encryption7_aad_list : l:list uint8{List.Tot.length l == size_test1_encryption7_aad} =
-  [@inline_let]
-  let l = [
-    u8 0x43; u8 0x6f; u8 0x75; u8 0x6e; u8 0x74;
-    u8 0x2d; u8 0x37;
-  ] in
-  assert_norm(List.Tot.length l == size_test1_encryption7_aad);
-  l
-let test1_encryption7_aad : lbytes size_test1_encryption7_aad = createL test1_encryption7_aad_list
-
-// generated: "e4ac909e74ca97d420374dba157678aad8f335b5cdaac2ca2e1813f2b3a6c0f6cfbc690dfd9b04a140861b910b"
-inline_for_extraction
-let size_test1_encryption7_ciphertext: size_nat = 45
-let test1_encryption7_ciphertext_list : l:list uint8{List.Tot.length l == size_test1_encryption7_ciphertext} =
-  [@inline_let]
-  let l = [
-    u8 0xe4; u8 0xac; u8 0x90; u8 0x9e; u8 0x74;
-    u8 0xca; u8 0x97; u8 0xd4; u8 0x20; u8 0x37;
-    u8 0x4d; u8 0xba; u8 0x15; u8 0x76; u8 0x78;
-    u8 0xaa; u8 0xd8; u8 0xf3; u8 0x35; u8 0xb5;
-    u8 0xcd; u8 0xaa; u8 0xc2; u8 0xca; u8 0x2e;
-    u8 0x18; u8 0x13; u8 0xf2; u8 0xb3; u8 0xa6;
-    u8 0xc0; u8 0xf6; u8 0xcf; u8 0xbc; u8 0x69;
-    u8 0x0d; u8 0xfd; u8 0x9b; u8 0x04; u8 0xa1;
-    u8 0x40; u8 0x86; u8 0x1b; u8 0x91; u8 0x0b;
-  ] in
-  assert_norm(List.Tot.length l == size_test1_encryption7_ciphertext);
-  l
-let test1_encryption7_ciphertext : lbytes size_test1_encryption7_ciphertext = createL test1_encryption7_ciphertext_list
-
-// generated: "2764228860619e140920c7d0"
-inline_for_extraction
-let size_test1_encryption7_nonce: size_nat = 12
-let test1_encryption7_nonce_list : l:list uint8{List.Tot.length l == size_test1_encryption7_nonce} =
-  [@inline_let]
-  let l = [
-    u8 0x27; u8 0x64; u8 0x22; u8 0x88; u8 0x60;
-    u8 0x61; u8 0x9e; u8 0x14; u8 0x09; u8 0x20;
-    u8 0xc7; u8 0xd0;
-  ] in
-  assert_norm(List.Tot.length l == size_test1_encryption7_nonce);
-  l
-let test1_encryption7_nonce : lbytes size_test1_encryption7_nonce = createL test1_encryption7_nonce_list
-
-// generated: "4265617574792069732074727574682c20747275746820626561757479"
-inline_for_extraction
-let size_test1_encryption7_plaintext: size_nat = 29
-let test1_encryption7_plaintext_list : l:list uint8{List.Tot.length l == size_test1_encryption7_plaintext} =
-  [@inline_let]
-  let l = [
-    u8 0x42; u8 0x65; u8 0x61; u8 0x75; u8 0x74;
-    u8 0x79; u8 0x20; u8 0x69; u8 0x73; u8 0x20;
-    u8 0x74; u8 0x72; u8 0x75; u8 0x74; u8 0x68;
-    u8 0x2c; u8 0x20; u8 0x74; u8 0x72; u8 0x75;
-    u8 0x74; u8 0x68; u8 0x20; u8 0x62; u8 0x65;
-    u8 0x61; u8 0x75; u8 0x74; u8 0x79;
-  ] in
-  assert_norm(List.Tot.length l == size_test1_encryption7_plaintext);
-  l
-let test1_encryption7_plaintext : lbytes size_test1_encryption7_plaintext = createL test1_encryption7_plaintext_list
-
-// generated: "436f756e742d38"
-inline_for_extraction
-let size_test1_encryption8_aad: size_nat = 7
-let test1_encryption8_aad_list : l:list uint8{List.Tot.length l == size_test1_encryption8_aad} =
-  [@inline_let]
-  let l = [
-    u8 0x43; u8 0x6f; u8 0x75; u8 0x6e; u8 0x74;
-    u8 0x2d; u8 0x38;
-  ] in
-  assert_norm(List.Tot.length l == size_test1_encryption8_aad);
-  l
-let test1_encryption8_aad : lbytes size_test1_encryption8_aad = createL test1_encryption8_aad_list
-
-// generated: "bd664ef7fa8fd4ba23430453914ffa75c54c24a593d894ad6626635ef38792cf505b7925d2f8dcdc744b8a8acd"
-inline_for_extraction
-let size_test1_encryption8_ciphertext: size_nat = 45
-let test1_encryption8_ciphertext_list : l:list uint8{List.Tot.length l == size_test1_encryption8_ciphertext} =
-  [@inline_let]
-  let l = [
-    u8 0xbd; u8 0x66; u8 0x4e; u8 0xf7; u8 0xfa;
-    u8 0x8f; u8 0xd4; u8 0xba; u8 0x23; u8 0x43;
-    u8 0x04; u8 0x53; u8 0x91; u8 0x4f; u8 0xfa;
-    u8 0x75; u8 0xc5; u8 0x4c; u8 0x24; u8 0xa5;
-    u8 0x93; u8 0xd8; u8 0x94; u8 0xad; u8 0x66;
-    u8 0x26; u8 0x63; u8 0x5e; u8 0xf3; u8 0x87;
-    u8 0x92; u8 0xcf; u8 0x50; u8 0x5b; u8 0x79;
-    u8 0x25; u8 0xd2; u8 0xf8; u8 0xdc; u8 0xdc;
-    u8 0x74; u8 0x4b; u8 0x8a; u8 0x8a; u8 0xcd;
-  ] in
-  assert_norm(List.Tot.length l == size_test1_encryption8_ciphertext);
-  l
-let test1_encryption8_ciphertext : lbytes size_test1_encryption8_ciphertext = createL test1_encryption8_ciphertext_list
-
-// generated: "2764228860619e140920c7df"
-inline_for_extraction
-let size_test1_encryption8_nonce: size_nat = 12
-let test1_encryption8_nonce_list : l:list uint8{List.Tot.length l == size_test1_encryption8_nonce} =
-  [@inline_let]
-  let l = [
-    u8 0x27; u8 0x64; u8 0x22; u8 0x88; u8 0x60;
-    u8 0x61; u8 0x9e; u8 0x14; u8 0x09; u8 0x20;
-    u8 0xc7; u8 0xdf;
-  ] in
-  assert_norm(List.Tot.length l == size_test1_encryption8_nonce);
-  l
-let test1_encryption8_nonce : lbytes size_test1_encryption8_nonce = createL test1_encryption8_nonce_list
-
-// generated: "4265617574792069732074727574682c20747275746820626561757479"
-inline_for_extraction
-let size_test1_encryption8_plaintext: size_nat = 29
-let test1_encryption8_plaintext_list : l:list uint8{List.Tot.length l == size_test1_encryption8_plaintext} =
-  [@inline_let]
-  let l = [
-    u8 0x42; u8 0x65; u8 0x61; u8 0x75; u8 0x74;
-    u8 0x79; u8 0x20; u8 0x69; u8 0x73; u8 0x20;
-    u8 0x74; u8 0x72; u8 0x75; u8 0x74; u8 0x68;
-    u8 0x2c; u8 0x20; u8 0x74; u8 0x72; u8 0x75;
-    u8 0x74; u8 0x68; u8 0x20; u8 0x62; u8 0x65;
-    u8 0x61; u8 0x75; u8 0x74; u8 0x79;
-  ] in
-  assert_norm(List.Tot.length l == size_test1_encryption8_plaintext);
-  l
-let test1_encryption8_plaintext : lbytes size_test1_encryption8_plaintext = createL test1_encryption8_plaintext_list
-
-// generated: "436f756e742d39"
-inline_for_extraction
-let size_test1_encryption9_aad: size_nat = 7
-let test1_encryption9_aad_list : l:list uint8{List.Tot.length l == size_test1_encryption9_aad} =
-  [@inline_let]
-  let l = [
-    u8 0x43; u8 0x6f; u8 0x75; u8 0x6e; u8 0x74;
-    u8 0x2d; u8 0x39;
-  ] in
-  assert_norm(List.Tot.length l == size_test1_encryption9_aad);
-  l
-let test1_encryption9_aad : lbytes size_test1_encryption9_aad = createL test1_encryption9_aad_list
-
-// generated: "4b7f4832efecd0a808a367e4d2ac970d6604026e4386211c22912567a061a2558de77f7cb760f1837f6d048d71"
-inline_for_extraction
-let size_test1_encryption9_ciphertext: size_nat = 45
-let test1_encryption9_ciphertext_list : l:list uint8{List.Tot.length l == size_test1_encryption9_ciphertext} =
-  [@inline_let]
-  let l = [
-    u8 0x4b; u8 0x7f; u8 0x48; u8 0x32; u8 0xef;
-    u8 0xec; u8 0xd0; u8 0xa8; u8 0x08; u8 0xa3;
-    u8 0x67; u8 0xe4; u8 0xd2; u8 0xac; u8 0x97;
-    u8 0x0d; u8 0x66; u8 0x04; u8 0x02; u8 0x6e;
-    u8 0x43; u8 0x86; u8 0x21; u8 0x1c; u8 0x22;
-    u8 0x91; u8 0x25; u8 0x67; u8 0xa0; u8 0x61;
-    u8 0xa2; u8 0x55; u8 0x8d; u8 0xe7; u8 0x7f;
-    u8 0x7c; u8 0xb7; u8 0x60; u8 0xf1; u8 0x83;
-    u8 0x7f; u8 0x6d; u8 0x04; u8 0x8d; u8 0x71;
-  ] in
-  assert_norm(List.Tot.length l == size_test1_encryption9_ciphertext);
-  l
-let test1_encryption9_ciphertext : lbytes size_test1_encryption9_ciphertext = createL test1_encryption9_ciphertext_list
-
-// generated: "2764228860619e140920c7de"
-inline_for_extraction
-let size_test1_encryption9_nonce: size_nat = 12
-let test1_encryption9_nonce_list : l:list uint8{List.Tot.length l == size_test1_encryption9_nonce} =
-  [@inline_let]
-  let l = [
-    u8 0x27; u8 0x64; u8 0x22; u8 0x88; u8 0x60;
-    u8 0x61; u8 0x9e; u8 0x14; u8 0x09; u8 0x20;
-    u8 0xc7; u8 0xde;
-  ] in
-  assert_norm(List.Tot.length l == size_test1_encryption9_nonce);
-  l
-let test1_encryption9_nonce : lbytes size_test1_encryption9_nonce = createL test1_encryption9_nonce_list
-
-// generated: "4265617574792069732074727574682c20747275746820626561757479"
-inline_for_extraction
-let size_test1_encryption9_plaintext: size_nat = 29
-let test1_encryption9_plaintext_list : l:list uint8{List.Tot.length l == size_test1_encryption9_plaintext} =
-  [@inline_let]
-  let l = [
-    u8 0x42; u8 0x65; u8 0x61; u8 0x75; u8 0x74;
-    u8 0x79; u8 0x20; u8 0x69; u8 0x73; u8 0x20;
-    u8 0x74; u8 0x72; u8 0x75; u8 0x74; u8 0x68;
-    u8 0x2c; u8 0x20; u8 0x74; u8 0x72; u8 0x75;
-    u8 0x74; u8 0x68; u8 0x20; u8 0x62; u8 0x65;
-    u8 0x61; u8 0x75; u8 0x74; u8 0x79;
-  ] in
-  assert_norm(List.Tot.length l == size_test1_encryption9_plaintext);
-  l
-let test1_encryption9_plaintext : lbytes size_test1_encryption9_plaintext = createL test1_encryption9_plaintext_list
-
-// generated: "436f6e746578742d30"
-inline_for_extraction
-let size_test1_export0_exportContext: size_nat = 9
-let test1_export0_exportContext_list : l:list uint8{List.Tot.length l == size_test1_export0_exportContext} =
-  [@inline_let]
-  let l = [
-    u8 0x43; u8 0x6f; u8 0x6e; u8 0x74; u8 0x65;
-    u8 0x78; u8 0x74; u8 0x2d; u8 0x30;
-  ] in
-  assert_norm(List.Tot.length l == size_test1_export0_exportContext);
-  l
-let test1_export0_exportContext : lbytes size_test1_export0_exportContext = createL test1_export0_exportContext_list
-
-// generated: "76d8f9425846916bf678504e398e984d91878220f34c5a5e1a63ac75ba0176bc"
-inline_for_extraction
-let size_test1_export0_exportValue: size_nat = 32
-let test1_export0_exportValue_list : l:list uint8{List.Tot.length l == size_test1_export0_exportValue} =
-  [@inline_let]
-  let l = [
-    u8 0x76; u8 0xd8; u8 0xf9; u8 0x42; u8 0x58;
-    u8 0x46; u8 0x91; u8 0x6b; u8 0xf6; u8 0x78;
-    u8 0x50; u8 0x4e; u8 0x39; u8 0x8e; u8 0x98;
-    u8 0x4d; u8 0x91; u8 0x87; u8 0x82; u8 0x20;
-    u8 0xf3; u8 0x4c; u8 0x5a; u8 0x5e; u8 0x1a;
-    u8 0x63; u8 0xac; u8 0x75; u8 0xba; u8 0x01;
-    u8 0x76; u8 0xbc;
-  ] in
-  assert_norm(List.Tot.length l == size_test1_export0_exportValue);
-  l
-let test1_export0_exportValue : lbytes size_test1_export0_exportValue = createL test1_export0_exportValue_list
-
-let test1_export0_len:size_nat = 32
-// generated: "436f6e746578742d31"
-inline_for_extraction
-let size_test1_export1_exportContext: size_nat = 9
-let test1_export1_exportContext_list : l:list uint8{List.Tot.length l == size_test1_export1_exportContext} =
-  [@inline_let]
-  let l = [
-    u8 0x43; u8 0x6f; u8 0x6e; u8 0x74; u8 0x65;
-    u8 0x78; u8 0x74; u8 0x2d; u8 0x31;
-  ] in
-  assert_norm(List.Tot.length l == size_test1_export1_exportContext);
-  l
-let test1_export1_exportContext : lbytes size_test1_export1_exportContext = createL test1_export1_exportContext_list
-
-// generated: "94fe3245047dde534862778ca1962e594b1758df5a525b4caa54ff0feadad06b"
-inline_for_extraction
-let size_test1_export1_exportValue: size_nat = 32
-let test1_export1_exportValue_list : l:list uint8{List.Tot.length l == size_test1_export1_exportValue} =
-  [@inline_let]
-  let l = [
-    u8 0x94; u8 0xfe; u8 0x32; u8 0x45; u8 0x04;
-    u8 0x7d; u8 0xde; u8 0x53; u8 0x48; u8 0x62;
-    u8 0x77; u8 0x8c; u8 0xa1; u8 0x96; u8 0x2e;
-    u8 0x59; u8 0x4b; u8 0x17; u8 0x58; u8 0xdf;
-    u8 0x5a; u8 0x52; u8 0x5b; u8 0x4c; u8 0xaa;
-    u8 0x54; u8 0xff; u8 0x0f; u8 0xea; u8 0xda;
-    u8 0xd0; u8 0x6b;
-  ] in
-  assert_norm(List.Tot.length l == size_test1_export1_exportValue);
-  l
-let test1_export1_exportValue : lbytes size_test1_export1_exportValue = createL test1_export1_exportValue_list
-
-let test1_export1_len:size_nat = 32
-// generated: "436f6e746578742d32"
-inline_for_extraction
-let size_test1_export2_exportContext: size_nat = 9
-let test1_export2_exportContext_list : l:list uint8{List.Tot.length l == size_test1_export2_exportContext} =
-  [@inline_let]
-  let l = [
-    u8 0x43; u8 0x6f; u8 0x6e; u8 0x74; u8 0x65;
-    u8 0x78; u8 0x74; u8 0x2d; u8 0x32;
-  ] in
-  assert_norm(List.Tot.length l == size_test1_export2_exportContext);
-  l
-let test1_export2_exportContext : lbytes size_test1_export2_exportContext = createL test1_export2_exportContext_list
-
-// generated: "97f0c64128ff1379af9ec623cba204b50cd9db9a6b7d90e7a28fed06badf363e"
-inline_for_extraction
-let size_test1_export2_exportValue: size_nat = 32
-let test1_export2_exportValue_list : l:list uint8{List.Tot.length l == size_test1_export2_exportValue} =
-  [@inline_let]
-  let l = [
-    u8 0x97; u8 0xf0; u8 0xc6; u8 0x41; u8 0x28;
-    u8 0xff; u8 0x13; u8 0x79; u8 0xaf; u8 0x9e;
-    u8 0xc6; u8 0x23; u8 0xcb; u8 0xa2; u8 0x04;
-    u8 0xb5; u8 0x0c; u8 0xd9; u8 0xdb; u8 0x9a;
-    u8 0x6b; u8 0x7d; u8 0x90; u8 0xe7; u8 0xa2;
-    u8 0x8f; u8 0xed; u8 0x06; u8 0xba; u8 0xdf;
-    u8 0x36; u8 0x3e;
-  ] in
-  assert_norm(List.Tot.length l == size_test1_export2_exportValue);
-  l
-let test1_export2_exportValue : lbytes size_test1_export2_exportValue = createL test1_export2_exportValue_list
-
-let test1_export2_len:size_nat = 32
-// generated: "436f6e746578742d33"
-inline_for_extraction
-let size_test1_export3_exportContext: size_nat = 9
-let test1_export3_exportContext_list : l:list uint8{List.Tot.length l == size_test1_export3_exportContext} =
-  [@inline_let]
-  let l = [
-    u8 0x43; u8 0x6f; u8 0x6e; u8 0x74; u8 0x65;
-    u8 0x78; u8 0x74; u8 0x2d; u8 0x33;
-  ] in
-  assert_norm(List.Tot.length l == size_test1_export3_exportContext);
-  l
-let test1_export3_exportContext : lbytes size_test1_export3_exportContext = createL test1_export3_exportContext_list
-
-// generated: "9cd27f832e7271f82ae85c3404d7d06ab2a5bebb9354bc022b9f016d74bcdb2c"
-inline_for_extraction
-let size_test1_export3_exportValue: size_nat = 32
-let test1_export3_exportValue_list : l:list uint8{List.Tot.length l == size_test1_export3_exportValue} =
-  [@inline_let]
-  let l = [
-    u8 0x9c; u8 0xd2; u8 0x7f; u8 0x83; u8 0x2e;
-    u8 0x72; u8 0x71; u8 0xf8; u8 0x2a; u8 0xe8;
-    u8 0x5c; u8 0x34; u8 0x04; u8 0xd7; u8 0xd0;
-    u8 0x6a; u8 0xb2; u8 0xa5; u8 0xbe; u8 0xbb;
-    u8 0x93; u8 0x54; u8 0xbc; u8 0x02; u8 0x2b;
-    u8 0x9f; u8 0x01; u8 0x6d; u8 0x74; u8 0xbc;
-    u8 0xdb; u8 0x2c;
-  ] in
-  assert_norm(List.Tot.length l == size_test1_export3_exportValue);
-  l
-let test1_export3_exportValue : lbytes size_test1_export3_exportValue = createL test1_export3_exportValue_list
-
-let test1_export3_len:size_nat = 32
-// generated: "436f6e746578742d34"
-inline_for_extraction
-let size_test1_export4_exportContext: size_nat = 9
-let test1_export4_exportContext_list : l:list uint8{List.Tot.length l == size_test1_export4_exportContext} =
-  [@inline_let]
-  let l = [
-    u8 0x43; u8 0x6f; u8 0x6e; u8 0x74; u8 0x65;
-    u8 0x78; u8 0x74; u8 0x2d; u8 0x34;
-  ] in
-  assert_norm(List.Tot.length l == size_test1_export4_exportContext);
-  l
-let test1_export4_exportContext : lbytes size_test1_export4_exportContext = createL test1_export4_exportContext_list
-
-// generated: "74da0b06441dd2aca2a43d5ee4796158c9403f7037e93c50bcbd6ea4a1687c06"
-inline_for_extraction
-let size_test1_export4_exportValue: size_nat = 32
-let test1_export4_exportValue_list : l:list uint8{List.Tot.length l == size_test1_export4_exportValue} =
-  [@inline_let]
-  let l = [
-    u8 0x74; u8 0xda; u8 0x0b; u8 0x06; u8 0x44;
-    u8 0x1d; u8 0xd2; u8 0xac; u8 0xa2; u8 0xa4;
-    u8 0x3d; u8 0x5e; u8 0xe4; u8 0x79; u8 0x61;
-    u8 0x58; u8 0xc9; u8 0x40; u8 0x3f; u8 0x70;
-    u8 0x37; u8 0xe9; u8 0x3c; u8 0x50; u8 0xbc;
-    u8 0xbd; u8 0x6e; u8 0xa4; u8 0xa1; u8 0x68;
-    u8 0x7c; u8 0x06;
-  ] in
-  assert_norm(List.Tot.length l == size_test1_export4_exportValue);
-  l
-let test1_export4_exportValue : lbytes size_test1_export4_exportValue = createL test1_export4_exportValue_list
-
-let test1_export4_len:size_nat = 32
-
-let test1 () =
-  let res = test_setupBase test1_ciphersuite test1_skEm test1_pkEm test1_skRm test1_pkRm test1_info test1_enc test1_zz test1_key_schedule_context test1_secret test1_key test1_nonce test1_exporterSecret test1_encryption0_nonce test1_encryption1_nonce in
-  let seq0:HPKE.seq_aead_s test1_ciphersuite = 0 in
-  let enc_res0 = test_encryption test1_ciphersuite test1_key test1_nonce test1_exporterSecret test1_encryption0_aad test1_encryption0_plaintext seq0 test1_encryption0_ciphertext test1_encryption0_nonce in
+let test0 () =
+  assert (size_test0_key_schedule_context = HPKE.size_ks_ctx test0_ciphersuite);
+  let res = test_setupBase test0_ciphersuite test0_skEm test0_pkEm test0_skRm test0_pkRm test0_info test0_enc test0_shared_secret test0_key_schedule_context test0_secret test0_key test0_base_nonce test0_exporter_secret test0_encryption0_nonce test0_encryption1_nonce in
+  let seq0:HPKE.seq_aead_s test0_ciphersuite = 0 in
+  let enc_res0 = test_encryption test0_ciphersuite test0_key test0_base_nonce test0_exporter_secret test0_encryption0_aad test0_encryption0_plaintext seq0 test0_encryption0_ciphertext test0_encryption0_nonce in
 
   assert_norm (1 < pow2 (8 * 12));
-  let seq1:HPKE.seq_aead_s test1_ciphersuite = (seq0 + 1) in
-  let enc_res1 = test_encryption test1_ciphersuite test1_key test1_nonce test1_exporterSecret test1_encryption1_aad test1_encryption1_plaintext seq1 test1_encryption1_ciphertext test1_encryption1_nonce in
+  let seq1:HPKE.seq_aead_s test0_ciphersuite = (seq0 + 1) in
+  let enc_res1 = test_encryption test0_ciphersuite test0_key test0_base_nonce test0_exporter_secret test0_encryption1_aad test0_encryption1_plaintext seq1 test0_encryption1_ciphertext test0_encryption1_nonce in
 
-  assert_norm (2 < pow2 (8 * 12));
-  let seq2:HPKE.seq_aead_s test1_ciphersuite = (seq1 + 1) in
-  let enc_res2 = test_encryption test1_ciphersuite test1_key test1_nonce test1_exporterSecret test1_encryption2_aad test1_encryption2_plaintext 2 test1_encryption2_ciphertext test1_encryption2_nonce in
 
-  assert_norm (3 < pow2 (8 * 12));
-  let seq3:HPKE.seq_aead_s test1_ciphersuite = (seq2 + 1) in
-  let enc_res3 = test_encryption test1_ciphersuite test1_key test1_nonce test1_exporterSecret test1_encryption3_aad test1_encryption3_plaintext 3 test1_encryption3_ciphertext test1_encryption3_nonce in
+  let exp_res0 = test_export test0_ciphersuite test0_key test0_base_nonce test0_exporter_secret test0_export0_exporter_context test0_export0_len test0_export0_exported_value in
 
-  assert_norm (4 < pow2 (8 * 12));
-  let seq4:HPKE.seq_aead_s test1_ciphersuite = (seq3 + 1) in
-  let enc_res4 = test_encryption test1_ciphersuite test1_key test1_nonce test1_exporterSecret test1_encryption4_aad test1_encryption4_plaintext 4 test1_encryption4_ciphertext test1_encryption4_nonce in
+  let exp_res1 = test_export test0_ciphersuite test0_key test0_base_nonce test0_exporter_secret test0_export1_exporter_context test0_export1_len test0_export1_exported_value in
 
-  assert_norm (5 < pow2 (8 * 12));
-  let seq5:HPKE.seq_aead_s test1_ciphersuite = (seq4 + 1) in
-  let enc_res5 = test_encryption test1_ciphersuite test1_key test1_nonce test1_exporterSecret test1_encryption5_aad test1_encryption5_plaintext 5 test1_encryption5_ciphertext test1_encryption5_nonce in
-
-  assert_norm (6 < pow2 (8 * 12));
-  let seq6:HPKE.seq_aead_s test1_ciphersuite = (seq5 + 1) in
-  let enc_res6 = test_encryption test1_ciphersuite test1_key test1_nonce test1_exporterSecret test1_encryption6_aad test1_encryption6_plaintext 6 test1_encryption6_ciphertext test1_encryption6_nonce in
-
-  assert_norm (7 < pow2 (8 * 12));
-  let seq7:HPKE.seq_aead_s test1_ciphersuite = (seq6 + 1) in
-  let enc_res7 = test_encryption test1_ciphersuite test1_key test1_nonce test1_exporterSecret test1_encryption7_aad test1_encryption7_plaintext 7 test1_encryption7_ciphertext test1_encryption7_nonce in
-
-  assert_norm (8 < pow2 (8 * 12));
-  let seq8:HPKE.seq_aead_s test1_ciphersuite = (seq7 + 1) in
-  let enc_res8 = test_encryption test1_ciphersuite test1_key test1_nonce test1_exporterSecret test1_encryption8_aad test1_encryption8_plaintext 8 test1_encryption8_ciphertext test1_encryption8_nonce in
-
-  assert_norm (9 < pow2 (8 * 12));
-  let seq9:HPKE.seq_aead_s test1_ciphersuite = (seq8 + 1) in
-  let enc_res9 = test_encryption test1_ciphersuite test1_key test1_nonce test1_exporterSecret test1_encryption9_aad test1_encryption9_plaintext 9 test1_encryption9_ciphertext test1_encryption9_nonce in
-
-  let exp_res0 = test_export test1_ciphersuite test1_key test1_nonce test1_exporterSecret test1_export0_exportContext test1_export0_len test1_export0_exportValue in
-
-  let exp_res1 = test_export test1_ciphersuite test1_key test1_nonce test1_exporterSecret test1_export1_exportContext test1_export1_len test1_export1_exportValue in
-
-  let exp_res2 = test_export test1_ciphersuite test1_key test1_nonce test1_exporterSecret test1_export2_exportContext test1_export2_len test1_export2_exportValue in
-
-  let exp_res3 = test_export test1_ciphersuite test1_key test1_nonce test1_exporterSecret test1_export3_exportContext test1_export3_len test1_export3_exportValue in
-
-  let exp_res4 = test_export test1_ciphersuite test1_key test1_nonce test1_exporterSecret test1_export4_exportContext test1_export4_len test1_export4_exportValue in
-
-  enc_res0 && enc_res1 && enc_res2 && enc_res3 && enc_res4 && enc_res5 && enc_res6 && enc_res7 && enc_res8 && enc_res9 && res && exp_res0 && exp_res1 && exp_res2 && exp_res3 && exp_res4
+  enc_res0 && enc_res1 && res && exp_res0 && exp_res1
 
 
 //
@@ -1166,7 +552,7 @@ let test1 () =
 
 
 let test () =
-  let r1  = test1  () in
+  let r1  = test0  () in
   (* let r4  = test4  () in *)
   (* let r8  = test8  () in *)
   (* let r14 = test14 () in *)
@@ -1204,3 +590,5 @@ let test () =
   (* let max_length_exp_ctx (cs:ciphersuite) = labeled_expand_max_length_info cs size_label_sec *)
   r1
   (* && r4 && r8 && r14 && r16 && r20 && r50 && r52 && r56 && r60 && r66 && r70 *)
+
+(* Execute it using make in the hacl-star root directory test-ml-Spec_HPKE_Test *)
